updated top-level logic

atomics/general_atomics.v
@@ -20,8 +20,8 @@ Definition atomic_shift {A B} (a : A -> mpred) Ei Eo (b : A -> B -> mpred) (Q : 
   @atomic_update mpredI _ [tele _ : A] [tele _ : B] Eo Ei (λ.. x, a (tele_unwrap x)) (λ.. x y, b (tele_unwrap x) (tele_unwrap y)) (λ.. x y, Q (tele_unwrap y)).
 
 Lemma atomic_commit_fupd : forall {A B} (a : A -> mpred) Ei Eo (b : A -> B -> mpred) (Q : B -> mpred) R R',
-  (forall x, R * a x |-- (|==> (EX y, b x y * R' y))%I) ->
-  (atomic_shift a Ei Eo b Q * R |-- |={Eo}=> (EX y, Q y * R' y))%I.
+  (forall x, R * a x |-- |==> (EX y, b x y * R' y)) ->
+  atomic_shift a Ei Eo b Q * R |-- |={Eo}=> (EX y, Q y * R' y).
 Proof.
   intros.
   iIntros "[AS R]".
@@ -31,30 +31,9 @@ Proof.
   iExists y; iMod ("commit" with "b") as "$"; auto.
 Qed.
 
-Corollary atomic_commit_elim : forall {A B} (a : A -> mpred) Ei Eo (b : A -> B -> mpred) (Q : B -> mpred) R R',
-  (forall x, R * a x |-- (|==> (EX y, b x y * R' y))%I) ->
-  (wsat * ghost_set g_en (coPset_to_Ensemble Eo) * atomic_shift a Ei Eo b Q * R |-- |==> ◇ (wsat * ghost_set g_en (coPset_to_Ensemble Eo) * (EX y, Q y * R' y)))%I.
-Proof.
-  intros.
-  iIntros "[[[wsat en] AS] R]".
-  iApply wsat_fupd_elim'; iFrame.
-  iApply atomic_commit_fupd; eauto; iFrame.
-Qed.
-
-(*(* This is unsound: what we really need is fupd in WP.
-   But that might not be necessary if we use atomic specs for all concurrent operations. *)
-Lemma atomic_commit : forall {A B} (a : A -> mpred) Ei Eo (b : A -> B -> mpred) (Q : B -> mpred) R R',
-  (forall x, R * a x |-- (|==> (EX y, b x y * R' y))%I) ->
-  (atomic_shift a Ei Eo b Q * R |-- |==> (EX y, Q y * R' y))%I.
-Proof.
-  intros.
-  eapply atomic_commit_elim in H.
-  admit.
-Admitted.*)
-
 Lemma atomic_rollback_fupd : forall {A B} (a : A -> mpred) Ei Eo (b : A -> B -> mpred) (Q : B -> mpred) R R',
-  (forall x, R * a x |-- (|==> a x * R')%I) ->
-  (atomic_shift a Ei Eo b Q * R |-- |={Eo}=> atomic_shift a Ei Eo b Q * R')%I.
+  (forall x, R * a x |-- |==> a x * R') ->
+  atomic_shift a Ei Eo b Q * R |-- |={Eo}=> atomic_shift a Ei Eo b Q * R'.
 Proof.
   intros.
   iIntros "[AS R]".
@@ -64,25 +43,6 @@ Proof.
   iMod ("rollback" with "a") as "$"; auto.
 Qed.
 
-Corollary atomic_rollback_elim : forall {A B} (a : A -> mpred) Ei Eo (b : A -> B -> mpred) (Q : B -> mpred) R R',
-  (forall x, R * a x |-- (|==> a x * R')%I) ->
-  (wsat * ghost_set g_en (coPset_to_Ensemble Eo) * atomic_shift a Ei Eo b Q * R |-- |==> ◇ (wsat * ghost_set g_en (coPset_to_Ensemble Eo) * (atomic_shift a Ei Eo b Q * R')))%I.
-Proof.
-  intros.
-  iIntros "[[[wsat en] AS] R]".
-  iApply wsat_fupd_elim'; iFrame "wsat en".
-  iApply atomic_rollback_fupd; eauto; iFrame.
-Qed.
-
-(*Lemma atomic_rollback : forall {A B} (a : A -> mpred) Ei Eo (b : A -> B -> mpred) (Q : B -> mpred) R R',
-  (forall x, R * a x |-- (|==> a x * R')%I) ->
-  (atomic_shift a Ei Eo b Q * R |-- atomic_shift a Ei Eo b Q * R')%I.
-Proof.
-  intros.
-  eapply atomic_rollback_elim in H.
-  admit.
-Admitted.*)
-
 Lemma atomic_shift_mask_weaken {A B} Eo1 Eo2 Ei a (b : A -> B -> mpred) Q :
   Eo1 ⊆ Eo2 ->
   atomic_shift a Ei Eo1 b Q |-- atomic_shift a Ei Eo2 b Q.
@@ -91,26 +51,26 @@ Proof.
   apply atomic_update_mask_weaken; auto.
 Qed.
 
-(* might be able to get rid of this if we do iInv instances *)
+(* use iInv instead of applying this lemma *)
 Lemma inv_atomic_shift : forall {A B} a Ei Eo (b : A -> B -> mpred) Q i R P
-  (Hi : inv i ⊆ Eo) (Hio : Ei ⊆ Eo ∖ inv i)
-  (Ha1 : (invariant i R * |>R |-- |={Eo ∖ inv i}=> EX x, a x * ((a x -* |={Ei}=> |>R) &&
-    (ALL y, |> P * b x y -* |={Ei}=> |>R * Q y)))%I),
-  invariant i R * |> P |-- atomic_shift a Ei Eo b Q.
+  (Hi : to_coPset i ⊆ Eo) (Hio : Ei ⊆ Eo ∖ to_coPset i)
+  (Ha1 : (inv i R * |>R |-- |={Eo ∖ to_coPset i}=> EX x, a x * ((a x -* |={Ei}=> |>R) &&
+    (ALL y, |> P * b x y -* |={Ei}=> |>R * Q y)))),
+  inv i R * |> P |-- atomic_shift a Ei Eo b Q.
 Proof.
   intros; unfold atomic_shift.
   iIntros "[#I P]". iAuIntro.
   rewrite /atomic_acc /=.
-  iMod (inv_open with "I") as "[R Hclose]"; first done.
+  iInv "I" as "R" "Hclose".
   iMod (Ha1 with "[$I $R]") as (x) "(a & shift)".
-  iExists x; iFrame "a".
-  iMod fupd_mask_subseteq as "mask"; first done.
-  iIntros "!>"; iSplit.
+  iExists x; iFrame.
+  iApply fupd_mask_intro; first done.
+  iIntros "Hclose'"; iSplit.
   - iIntros "a"; iMod ("shift" with "a") as "R".
-    iMod "mask"; iMod ("Hclose" with "R"); auto.
+    iMod "Hclose'"; iMod ("Hclose" with "R"); auto.
   - iIntros (y) "b".
     iMod ("shift" with "[$P $b]") as "[R Q]".
-    iMod "mask"; iMod ("Hclose" with "R"); auto.
+    iMod "Hclose'"; iMod ("Hclose" with "R"); auto.
 Qed.
 
 Lemma atomic_shift_nonexpansive : forall {A B} n a Ei Eo (b : A -> B -> mpred) Q,
@@ -141,7 +101,7 @@ Qed.
 Lemma atomic_shift_derives_frame : forall {A A' B B'} (a : A -> mpred) (a' : A' -> mpred) Ei Eo
   (b : A -> B -> mpred) (b' : A' -> B' -> mpred) (Q : B -> mpred) (Q' : B' -> mpred) R
   (Ha : (forall x, a x * |>R |-- |={Ei}=> EX x' : A', a' x' *
-    ((a' x' -* |={Ei}=> a x * |>R) && ALL y' : _, b' x' y' -* |={Ei}=> EX y : _, b x y * (Q y -* |={Eo}=> Q' y')))%I),
+    ((a' x' -* |={Ei}=> a x * |>R) && ALL y' : _, b' x' y' -* (|={Ei}=> EX y : _, b x y * (Q y -* |={Eo}=> Q' y'))))),
   atomic_shift a Ei Eo b Q * |>R |-- atomic_shift a' Ei Eo b' Q'.
 Proof.
   intros; unfold atomic_shift.
@@ -162,7 +122,7 @@ Qed.
 Lemma atomic_shift_derives : forall {A A' B B'} (a : A -> mpred) (a' : A' -> mpred) Ei Eo
   (b : A -> B -> mpred) (b' : A' -> B' -> mpred) (Q : B -> mpred) (Q' : B' -> mpred)
   (Ha : (forall x, a x  |-- |={Ei}=> EX x' : A', a' x' *
-    ((a' x' -* |={Ei}=> a x) && ALL y' : _, b' x' y' -* |={Ei}=> EX y : _, b x y * (Q y -* |={Eo}=> Q' y')))%I),
+    ((a' x' -* |={Ei}=> a x) && ALL y' : _, b' x' y' -* (|={Ei}=> EX y : _, b x y * (Q y -* |={Eo}=> Q' y'))))),
   atomic_shift a Ei Eo b Q |-- atomic_shift a' Ei Eo b' Q'.
 Proof.
   intros; unfold atomic_shift.
@@ -179,7 +139,7 @@ Qed.
 Lemma atomic_shift_derives' : forall {A A' B} (a : A -> mpred) (a' : A' -> mpred) Ei Eo
   (b : A -> B -> mpred) (b' : A' -> B -> mpred) (Q : B -> mpred)
   (Ha : (forall x, a x |-- |={Ei}=> EX x' : A', a' x' *
-    ((a' x' -* |={Ei}=> a x) && ALL y : _, b' x' y -* |={Ei}=> b x y))%I),
+    ((a' x' -* |={Ei}=> a x) && ALL y : _, b' x' y -* |={Ei}=> b x y))),
   atomic_shift a Ei Eo b Q |-- atomic_shift a' Ei Eo b' Q.
 Proof.
   intros; apply atomic_shift_derives.
@@ -194,9 +154,9 @@ Proof.
 Qed.
 
 Lemma atomic_shift_derives_simple : forall {A B} (a a' : A -> mpred) Ei Eo (b b' : A -> B -> mpred) (Q : B -> mpred)
-  (Ha1 : (forall x, a x |-- |={Ei}=> a' x)%I)
-  (Ha2 : (forall x, a' x |-- |={Ei}=> a x)%I)
-  (Hb : (forall x y, b' x y |-- |={Ei}=> b x y)%I),
+  (Ha1 : forall x, a x |-- |={Ei}=> a' x)
+  (Ha2 : forall x, a' x |-- |={Ei}=> a x)
+  (Hb : forall x y, b' x y |-- |={Ei}=> b x y),
   atomic_shift a Ei Eo b Q |-- atomic_shift a' Ei Eo b' Q.
 Proof.
   intros; apply atomic_shift_derives'; intros.
@@ -229,7 +189,7 @@ End atomicity.
 
 Global Hint Resolve empty_subseteq : core.
 
-Definition atomic_spec_type W T := ProdType W (ArrowType (ConstType T) Mpred)).
+Definition atomic_spec_type W T := ProdType W (ArrowType (ConstType T) Mpred).
 
 Definition super_non_expansive_a {A W} (a : forall ts : list Type, functors.MixVariantFunctor._functor
   (dependent_type_functor_rec ts W) (predicates_hered.pred rmap) -> A ts -> predicates_hered.pred rmap) :=
@@ -249,17 +209,17 @@ Import List.
 
 (* A is the type of the abstract data. T is the type quantified over in the postcondition.
    W is the TypeTree of the witness for the rest of the function. *)
-(*Notation atomic_spec1 T W args tz la P a t lb b Ei Eo :=
+(*Notation atomic_spec1 T W args tz la P a t lb b E :=
   (mk_funspec (pair args tz) cc_default (atomic_spec_type W T)
    (fun (ts: list Type) '(w, Q) =>
      PROP ()
      (LOCALx (map (fun l => l ts w) la)
-     (SEP (atomic_shift (a ts w) Ei Eo (b ts w) Q; P ts w))))
+     (SEP (atomic_shift (a ts w) (⊤ ∖ E) ∅ (b ts w) Q; P ts w))))
    (fun (ts: list Type) '(w, Q) => EX v : T,
      PROP () (LOCALx (map (fun l => l ts w v) lb)
      (SEP (Q v)))) _ _).*)
 
-Lemma atomic_spec_nonexpansive_pre' : forall {A T} {t : Inhabitant T} W P L G R S2 Ei Eo SQ
+Lemma atomic_spec_nonexpansive_pre' : forall {A T} {t : Inhabitant T} W P L G R S2 E SQ
   (HP : @super_non_expansive_list W (fun ts a _ => map prop (P ts a)))
   (HL: forall n ts x, L ts x = L ts (functors.MixVariantFunctor.fmap _ (compcert_rmaps.RML.R.approx n) (compcert_rmaps.RML.R.approx n) x))
   (HG: @super_non_expansive_list W (fun ts a rho => map (fun Q0 => prop (locald_denote (gvars Q0) rho)) (G ts a)))
@@ -270,28 +230,28 @@ Lemma atomic_spec_nonexpansive_pre' : forall {A T} {t : Inhabitant T} W P L G R 
   (fun ts (_a : functors.MixVariantFunctor._functor (dependent_type_functor_rec ts W) mpred * (T -> mpred)) =>
     let '(w, Q) := _a in
     PROPx (P ts w) (PARAMSx (L ts w) (GLOBALSx (G ts w)
-     (SEPx (atomic_shift(A := A ts) (S2 ts w) Ei Eo (SQ ts w) Q :: R ts w))))).
+     (SEPx (atomic_shift(A := A ts) (S2 ts w) (⊤ ∖ E) ∅ (SQ ts w) Q :: R ts w))))).
 Proof.
   intros.
   hnf; intros.
   etransitivity; [|etransitivity; [
-    apply (PROP_PARAMS_GLOBALS_SEP_args_super_non_expansive' (atomic_spec_type W T) (fun ts x => P ts (fst (fst x))) (fun ts x => L ts (fst (fst x))) (fun ts x => G ts (fst (fst x))) (fun ts '(w, Q) => atomic_shift(A := A ts) (S2 ts w) Ei Eo (SQ ts w) Q :: R ts w))|]].
-  - instantiate (9 := x). destruct x as ((?, ?), ?). reflexivity.
-  - intros ? ? ((?, ?), ?) ?; apply HP; auto.
-  - intros ? ? ((?, ?), ?); apply HL; auto.
-  - intros ? ? ((?, ?), ?); apply HG; auto.
-  - intros ? ? ((?, ?), ?) ?; constructor; [|apply HR; auto].
+    apply (PROP_PARAMS_GLOBALS_SEP_args_super_non_expansive' (atomic_spec_type W T) (fun ts x => P ts (fst x)) (fun ts x => L ts (fst x)) (fun ts x => G ts (fst x)) (fun ts '(w, Q) => atomic_shift(A := A ts) (S2 ts w) (⊤ ∖ E) ∅ (SQ ts w) Q :: R ts w))|]].
+  - instantiate (9 := x). destruct x. reflexivity.
+  - intros ? ? (?, ?) ?; apply HP; auto.
+  - intros ? ? (?, ?); apply HL; auto.
+  - intros ? ? (?, ?); apply HG; auto.
+  - intros ? ? (?, ?) ?; constructor; [|apply HR; auto].
     rewrite -> atomic_shift_nonexpansive by auto; setoid_rewrite atomic_shift_nonexpansive at 2; auto.
     f_equal; f_equal; repeat extensionality; simpl.
     + apply H.
     + apply H0.
     + rewrite approx_idem; auto.
-  - destruct x as ((?, ?), ?); reflexivity.
+  - destruct x as (?, ?); reflexivity.
 Qed.
 
 Definition atomic_spec_type0 W := ProdType W Mpred.
 
-Lemma atomic_spec_nonexpansive_pre0 : forall {A} W P L G R S2 Ei Eo SQ
+Lemma atomic_spec_nonexpansive_pre0 : forall {A} W P L G R S2 E SQ
   (HP : super_non_expansive_list (fun ts w _ => map prop (P ts w)))
   (HL: forall n ts x, L ts x = L ts (functors.MixVariantFunctor.fmap _ (compcert_rmaps.RML.R.approx n) (compcert_rmaps.RML.R.approx n) x))
   (HG: @super_non_expansive_list W (fun ts a rho => map (fun Q0 => prop (locald_denote (gvars Q0) rho)) (G ts a)))
@@ -302,30 +262,30 @@ Lemma atomic_spec_nonexpansive_pre0 : forall {A} W P L G R S2 Ei Eo SQ
   (fun ts (_a : functors.MixVariantFunctor._functor (dependent_type_functor_rec ts W) mpred * mpred) =>
     let '(w, Q) := _a in
     PROPx (P ts w) (PARAMSx (L ts w) (GLOBALSx (G ts w)
-     (SEPx (atomic_shift(A := A ts)(B := unit) (S2 ts w) Ei Eo (SQ ts w) (fun _ => Q) :: R ts w))))).
+     (SEPx (atomic_shift(A := A ts)(B := unit) (S2 ts w) (⊤ ∖ E) ∅ (SQ ts w) (fun _ => Q) :: R ts w))))).
 Proof.
   intros.
   hnf; intros.
   etransitivity; [|etransitivity; [
-    apply (PROP_PARAMS_GLOBALS_SEP_args_super_non_expansive' (atomic_spec_type0 W) (fun ts x => P ts (fst (fst x))) (fun ts x => L ts (fst (fst x))) (fun ts x => G ts (fst (fst x))) (fun ts '(w, Q) => atomic_shift(A := A ts) (S2 ts w) Ei Eo (SQ ts w) (fun _ => Q) :: R ts w))|]].
-  - instantiate (9 := x). destruct x as ((?, ?), ?). reflexivity.
-  - intros ? ? ((?, ?), ?) ?; apply HP; auto.
-  - intros ? ? ((?, ?), ?); apply HL; auto.
-  - intros ? ? ((?, ?), ?); apply HG; auto.
-  - intros ? ? ((?, ?), ?) ?; constructor; [|apply HR; auto].
+    apply (PROP_PARAMS_GLOBALS_SEP_args_super_non_expansive' (atomic_spec_type0 W) (fun ts x => P ts (fst x)) (fun ts x => L ts (fst x)) (fun ts x => G ts (fst x)) (fun ts '(w, Q) => atomic_shift(A := A ts) (S2 ts w) (⊤ ∖ E) ∅ (SQ ts w) (fun _ => Q) :: R ts w))|]].
+  - instantiate (9 := x). destruct x. reflexivity.
+  - intros ? ? (?, ?) ?; apply HP; auto.
+  - intros ? ? (?, ?); apply HL; auto.
+  - intros ? ? (?, ?); apply HG; auto.
+  - intros ? ? (?, ?) ?; constructor; [|apply HR; auto].
     rewrite -> atomic_shift_nonexpansive by auto; setoid_rewrite atomic_shift_nonexpansive at 2; auto.
     f_equal; f_equal; repeat extensionality; simpl.
     + apply H.
     + apply H0.
     + rewrite approx_idem; auto.
-  - destruct x as ((?, ?), ?); reflexivity.
+  - destruct x as (?, ?); reflexivity.
 Qed.
 
-Lemma atomic_spec_nonexpansive_pre : forall {A T} {t : Inhabitant T} W P L G R S2 Ei Eo SQ Pre
+Lemma atomic_spec_nonexpansive_pre : forall {A T} {t : Inhabitant T} W P L G R S2 E SQ Pre
   (Heq : (forall ts (_a : functors.MixVariantFunctor._functor (dependent_type_functor_rec ts W) mpred * (T -> mpred)),
    Pre ts _a = let '(w, Q) := _a in
     PROPx (P ts w) (PARAMSx (L ts w) (GLOBALSx (G ts w)
-     (SEPx (atomic_shift(A := A ts) (S2 ts w) Ei Eo (SQ ts w) Q :: R ts w))))))
+     (SEPx (atomic_shift(A := A ts) (S2 ts w) (⊤ ∖ E) ∅ (SQ ts w) Q :: R ts w))))))
   (HP : super_non_expansive_list (fun ts w _ => map prop (P ts w)))
   (HL: forall n ts x, L ts x = L ts (functors.MixVariantFunctor.fmap _ (compcert_rmaps.RML.R.approx n) (compcert_rmaps.RML.R.approx n) x))
   (HG: @super_non_expansive_list W (fun ts a rho => map (fun Q0 => prop (locald_denote (gvars Q0) rho)) (G ts a)))
@@ -354,11 +314,11 @@ Proof.
   destruct x as (w, Q).
   rewrite !approx_exp; f_equal; extensionality v.
   etransitivity; [|etransitivity; [
-    apply (PROP_LOCAL_SEP_super_non_expansive' (atomic_spec_type W T) (fun ts '(w, _, _) => []) (fun ts '(w, _, _) => L ts w v) (fun ts '(w, Q) => Q v :: R ts w v))|]].
+    apply (PROP_LOCAL_SEP_super_non_expansive' (atomic_spec_type W T) (fun ts '(w, _) => []) (fun ts '(w, _) => L ts w v) (fun ts '(w, Q) => Q v :: R ts w v))|]].
   - instantiate (1 := rho); instantiate (1 := ts); instantiate (1 := (w, Q)); reflexivity.
-  - intros ? ? ((?, ?), ?) ?; constructor.
-  - intros ? ? ((?, ?), ?) ?; apply HL; auto.
-  - intros ? ? ((?, ?), ?) ?; constructor; [|apply HR; auto].
+  - intros ? ? (?, ?) ?; constructor.
+  - intros ? ? (?, ?) ?; apply HL; auto.
+  - intros ? ? (?, ?) ?; constructor; [|apply HR; auto].
     simpl; rewrite approx_idem; auto.
   - reflexivity.
 Qed.
@@ -374,11 +334,11 @@ Proof.
   intros.
   hnf; intros.
   etransitivity; [|etransitivity; [
-    apply (PROP_LOCAL_SEP_super_non_expansive' (atomic_spec_type0 W) (fun ts '(w, _, _) => []) (fun ts '(w, _, _) => L ts w) (fun ts '(w, Q) => Q :: R ts w))|]].
-  - instantiate (1 := rho); instantiate (1 := ts); instantiate (1 := x); destruct x as ((?, ?), ?); reflexivity.
-  - intros ? ? ((?, ?), ?) ?; constructor.
-  - intros ? ? ((?, ?), ?) ?; apply HL; auto.
-  - intros ? ? ((?, ?), ?) ?; constructor; [|apply HR; auto].
+    apply (PROP_LOCAL_SEP_super_non_expansive' (atomic_spec_type0 W) (fun ts '(w, _) => []) (fun ts '(w, _) => L ts w) (fun ts '(w, Q) => Q :: R ts w))|]].
+  - instantiate (1 := rho); instantiate (1 := ts); instantiate (1 := x); destruct x as (?, ?); reflexivity.
+  - intros ? ? (?, ?) ?; constructor.
+  - intros ? ? (?, ?) ?; apply HL; auto.
+  - intros ? ? (?, ?) ?; constructor; [|apply HR; auto].
     simpl; rewrite approx_idem; auto.
   - reflexivity.
 Qed.
@@ -401,7 +361,7 @@ Qed.
 (* A is the type of the abstract data. T is the type quantified over in the postcondition.
    W is the TypeTree of the witness for the rest of the function. *)
 Program Definition atomic_spec {A T} {t : Inhabitant T} W args tz la P G Qp a lb
-        b Ei Eo
+        b E
    (HP : super_non_expansive' P) (HQp : forall v:T, super_non_expansive' (Qp v))
   (Ha : super_non_expansive_a(A := A) a) (Hla: forall n ts x, la ts x = la ts (functors.MixVariantFunctor.fmap _ (compcert_rmaps.RML.R.approx n) (compcert_rmaps.RML.R.approx n) x))
   (HG: @super_non_expansive_list W (fun ts a rho => map (fun Q0 => prop (locald_denote (gvars Q0) rho)) (G ts a)))
@@ -410,14 +370,14 @@ Program Definition atomic_spec {A T} {t : Inhabitant T} W args tz la P G Qp a lb
   (fun (ts: list Type) '(w, Q) =>
     PROP ()
     (PARAMSx (la ts w) (GLOBALSx (G ts w) (
-    (SEP (atomic_shift (a ts w) Ei Eo (b ts w) Q; P ts w))%assert5))))
+    (SEP (atomic_shift (a ts w) (⊤ ∖ E) ∅ (b ts w) Q; P ts w))%assert5))))
   (fun (ts: list Type) '(w, Q) => EX v : T,
     PROP () (LOCALx (lb ts w v)
     (SEP (Q v; Qp v ts w))%assert5)) _ _.
 Next Obligation.
 Proof.
   intros; eapply atomic_spec_nonexpansive_pre; try eassumption.
-  { intros ? ((?, ?), ?). reflexivity. }
+  { intros ? (?, ?). reflexivity. }
   all: auto.
   - constructor.
   - repeat constructor; repeat intro; auto.
@@ -425,17 +385,17 @@ Qed.
 Next Obligation.
 Proof.
   intros; eapply atomic_spec_nonexpansive_post.
-  { intros ? ((?, ?), ?); reflexivity. }
+  { intros ? (?, ?); reflexivity. }
   - auto.
   - repeat constructor.
     unfold super_non_expansive, super_non_expansive' in *.
     intros; apply HQp.
 Qed.
 
-Definition stable_spec_type W := ProdType (ProdType W
+(*Definition stable_spec_type W := ProdType (ProdType W
   (ArrowType (DependentType 0) (ArrowType (DependentType 1) Mpred))) (ArrowType (DependentType 1) Mpred).
 
-(*Lemma stabilize : forall T W args tz P1 P2 Q1 Q2 neP1 neP2 neQ1 neQ2
+Lemma stabilize : forall T W args tz P1 P2 Q1 Q2 neP1 neP2 neQ1 neQ2
   PP la P a lb b Ei Eo Q'
   (Hpre1 : forall ts w Q, P1 ts (w, Q) =
      PROP (PP ts w)
@@ -595,12 +555,12 @@ Definition tcurry_rev (A : tlist) : tuple_type_rev A -> tuple_type A
 Definition rev_curry {A B} (f : tuple_type A -> B) : tuple_type_rev A -> B
   := fun v => f (tcurry_rev _ v).
 
-Notation "'ATOMIC' 'TYPE' W 'OBJ' x : A 'INVS' Ei Eo 'WITH' x1 , .. , xn 'PRE'  [ u , .. , v ] 'PROP' ( Px ; .. ; Py ) 'PARAMS' ( Lx ; .. ; Ly ) 'GLOBALS' ( Gx ; .. ; Gy ) 'SEP' ( S1x ; .. ; S1y ) '|' S2 'POST' [ tz ] 'EX' r : T , 'PROP' () 'LOCAL' ( LQx ; .. ; LQy ) 'SEP' ( SPx ; .. ; SPy ) '|' ( SQx ; .. ; SQy )" :=
+Notation "'ATOMIC' 'TYPE' W 'OBJ' x : A 'INVS' E 'WITH' x1 , .. , xn 'PRE'  [ u , .. , v ] 'PROP' ( Px ; .. ; Py ) 'PARAMS' ( Lx ; .. ; Ly ) 'GLOBALS' ( Gx ; .. ; Gy ) 'SEP' ( S1x ; .. ; S1y ) '|' S2 'POST' [ tz ] 'EX' r : T , 'PROP' () 'LOCAL' ( LQx ; .. ; LQy ) 'SEP' ( SPx ; .. ; SPy ) '|' ( SQx ; .. ; SQy )" :=
   (mk_funspec (pair (cons u%type .. (cons v%type nil) ..) tz) cc_default (atomic_spec_type W T)
    (fun (ts: list Type) => rev_curry (tcurry (fun x1 => .. (tcurry (fun xn => tcurry (fun Q : (T -> mpred) => tcurry (fun (_ : tuple_type tnil) =>
      PROPx (cons Px%type .. (cons Py%type nil) ..)
      (PARAMSx (cons Lx%type .. (cons Ly%type nil) ..) (GLOBALSx (cons Gx .. (cons Gy nil) ..)
-     (SEPx (cons (atomic_shift (fun x => S2) Ei Eo (fun x r => fold_right_sepcon (cons SQx%logic .. (cons SQy%logic nil) ..)) Q) (cons S1x%logic .. (cons S1y%logic nil) ..))))))))) ..)))
+     (SEPx (cons (atomic_shift (fun x => S2) (⊤ ∖ E) ∅ (fun x r => fold_right_sepcon (cons SQx%logic .. (cons SQy%logic nil) ..)) Q) (cons S1x%logic .. (cons S1y%logic nil) ..))))))))) ..)))
    (fun (ts: list Type) => rev_curry (tcurry (fun x1 => .. (tcurry (fun xn => tcurry (fun Q : (T -> mpred) => tcurry (fun (_ : tuple_type tnil) =>
     @exp (environ -> mpred) _ T (fun r =>
      PROP () (LOCALx (cons LQx .. (cons LQy nil) ..) ((SEPx (Q r :: cons SPx .. (cons SPy nil) ..))))))))) ..)))
@@ -609,21 +569,20 @@ Notation "'ATOMIC' 'TYPE' W 'OBJ' x : A 'INVS' Ei Eo 'WITH' x1 , .. , xn 'PRE'  
       (fun (ts: list Type) => rev_curry (tcurry (fun x1 => .. (tcurry (fun xn (_ : tuple_type tnil) => (cons Lx%type .. (cons Ly%type nil) ..))) ..)))
       (fun (ts: list Type) => rev_curry (tcurry (fun x1 => .. (tcurry (fun xn (_ : tuple_type tnil) => (cons Gx .. (cons Gy nil) ..))) ..)))
       (fun (ts: list Type) => rev_curry (tcurry (fun x1 => .. (tcurry (fun xn (_ : tuple_type tnil) => (cons S1x%logic .. (cons S1y%logic nil) ..))) ..)))
-      (fun (ts: list Type) => rev_curry (tcurry (fun x1 => .. (tcurry (fun xn (_ : tuple_type tnil) x => S2)) ..)))
-      Ei Eo
+      (fun (ts: list Type) => rev_curry (tcurry (fun x1 => .. (tcurry (fun xn (_ : tuple_type tnil) x => S2)) ..))) E
       (fun (ts: list Type) => rev_curry (tcurry (fun x1 => .. (tcurry (fun xn (_ : tuple_type tnil) x r => fold_right_sepcon (cons SQx%logic .. (cons SQy%logic nil) ..))) ..)))
      _ _ _ _ _ _)
   (atomic_spec_nonexpansive_post' W
       (fun (ts: list Type) => rev_curry (tcurry (fun x1 => .. (tcurry (fun xn (_ : tuple_type tnil) r => (cons LQx%assert3 .. (cons LQy%assert3 nil) ..))) ..)))
       (fun (ts: list Type) => rev_curry (tcurry (fun x1 => .. (tcurry (fun xn (_ : tuple_type tnil) r => (cons SPx%assert3 .. (cons SPy%assert3 nil) ..))) ..))) _ _))
-  (at level 200, x1 closed binder, xn closed binder, x at level 0, Ei at level 0, Eo at level 0, S2 at level 0, r at level 0, T at level 0).
+  (at level 200, x1 closed binder, xn closed binder, x at level 0, E at level 0, S2 at level 0, r at level 0, T at level 0).
 
-Notation "'ATOMIC' 'TYPE' W 'OBJ' x 'INVS' Ei Eo 'WITH' x1 , .. , xn 'PRE'  [ u , .. , v ] 'PROP' ( Px ; .. ; Py ) 'PARAMS' ( Lx ; .. ; Ly ) 'GLOBALS' ( Gx ; .. ; Gy ) 'SEP' ( S1x ; .. ; S1y ) '|' S2 'POST' [ tz ] 'EX' r : T , 'PROP' () 'LOCAL' ( LQx ; .. ; LQy ) 'SEP' ( SPx ; .. ; SPy ) '|' ( SQx ; .. ; SQy )" :=
+Notation "'ATOMIC' 'TYPE' W 'OBJ' x 'INVS' E 'WITH' x1 , .. , xn 'PRE'  [ u , .. , v ] 'PROP' ( Px ; .. ; Py ) 'PARAMS' ( Lx ; .. ; Ly ) 'GLOBALS' ( Gx ; .. ; Gy ) 'SEP' ( S1x ; .. ; S1y ) '|' S2 'POST' [ tz ] 'EX' r : T , 'PROP' () 'LOCAL' ( LQx ; .. ; LQy ) 'SEP' ( SPx ; .. ; SPy ) '|' ( SQx ; .. ; SQy )" :=
   (mk_funspec (pair (cons u%type .. (cons v%type nil) ..) tz) cc_default (atomic_spec_type W T)
    (fun (ts: list Type) => rev_curry (tcurry (fun x1 => .. (tcurry (fun xn => tcurry (fun Q : (T -> mpred) => tcurry (fun (_ : tuple_type tnil) =>
      PROPx (cons Px%type .. (cons Py%type nil) ..)
      (PARAMSx (cons Lx%type .. (cons Ly%type nil) ..) (GLOBALSx (cons Gx .. (cons Gy nil) ..)
-     (SEPx (cons (atomic_shift (fun x => S2) Ei Eo (fun x r => fold_right_sepcon (cons SQx%logic .. (cons SQy%logic nil) ..)) Q) (cons S1x%logic .. (cons S1y%logic nil) ..))))))))) ..)))
+     (SEPx (cons (atomic_shift (fun x => S2) (⊤ ∖ E) ∅ (fun x r => fold_right_sepcon (cons SQx%logic .. (cons SQy%logic nil) ..)) Q) (cons S1x%logic .. (cons S1y%logic nil) ..))))))))) ..)))
    (fun (ts: list Type) => rev_curry (tcurry (fun x1 => .. (tcurry (fun xn => tcurry (fun Q : (T -> mpred) => tcurry (fun (_ : tuple_type tnil) =>
     @exp (environ -> mpred) _ T (fun r =>
      PROP () (LOCALx (cons LQx .. (cons LQy nil) ..) ((SEPx (Q r :: cons SPx .. (cons SPy nil) ..))))))))) ..)))
@@ -632,21 +591,20 @@ Notation "'ATOMIC' 'TYPE' W 'OBJ' x 'INVS' Ei Eo 'WITH' x1 , .. , xn 'PRE'  [ u 
       (fun (ts: list Type) => rev_curry (tcurry (fun x1 => .. (tcurry (fun xn (_ : tuple_type tnil) => (cons Lx%type .. (cons Ly%type nil) ..))) ..)))
       (fun (ts: list Type) => rev_curry (tcurry (fun x1 => .. (tcurry (fun xn (_ : tuple_type tnil) => (cons Gx .. (cons Gy nil) ..))) ..)))
       (fun (ts: list Type) => rev_curry (tcurry (fun x1 => .. (tcurry (fun xn (_ : tuple_type tnil) => (cons S1x%logic .. (cons S1y%logic nil) ..))) ..)))
-      (fun (ts: list Type) => rev_curry (tcurry (fun x1 => .. (tcurry (fun xn (_ : tuple_type tnil) x => S2)) ..)))
-      Ei Eo
+      (fun (ts: list Type) => rev_curry (tcurry (fun x1 => .. (tcurry (fun xn (_ : tuple_type tnil) x => S2)) ..))) E
       (fun (ts: list Type) => rev_curry (tcurry (fun x1 => .. (tcurry (fun xn (_ : tuple_type tnil) x r => fold_right_sepcon (cons SQx%logic .. (cons SQy%logic nil) ..))) ..)))
      _ _ _ _ _ _)
   (atomic_spec_nonexpansive_post' W
       (fun (ts: list Type) => rev_curry (tcurry (fun x1 => .. (tcurry (fun xn (_ : tuple_type tnil) r => (cons LQx%assert3 .. (cons LQy%assert3 nil) ..))) ..)))
       (fun (ts: list Type) => rev_curry (tcurry (fun x1 => .. (tcurry (fun xn (_ : tuple_type tnil) r => (cons SPx%assert3 .. (cons SPy%assert3 nil) ..))) ..))) _ _))
-  (at level 200, x1 closed binder, xn closed binder, x at level 0, Ei at level 0, Eo at level 0, S2 at level 0, r at level 0, T at level 0).
+  (at level 200, x1 closed binder, xn closed binder, x at level 0, E at level 0, S2 at level 0, r at level 0, T at level 0).
 
-Notation "'ATOMIC' 'TYPE' W 'OBJ' x 'INVS' Ei Eo 'WITH' x1 , .. , xn 'PRE'  [ u , .. , v ] 'PROP' ( Px ; .. ; Py ) 'PARAMS' ( Lx ; .. ; Ly ) 'GLOBALS' ( Gx ; .. ; Gy ) 'SEP' ( S1x ; .. ; S1y ) '|' S2 'POST' [ tz ] 'EX' r : T , 'PROP' () 'LOCAL' () 'SEP' ( SPx ; .. ; SPy ) '|' ( SQx ; .. ; SQy )" :=
+Notation "'ATOMIC' 'TYPE' W 'OBJ' x 'INVS' E 'WITH' x1 , .. , xn 'PRE'  [ u , .. , v ] 'PROP' ( Px ; .. ; Py ) 'PARAMS' ( Lx ; .. ; Ly ) 'GLOBALS' ( Gx ; .. ; Gy ) 'SEP' ( S1x ; .. ; S1y ) '|' S2 'POST' [ tz ] 'EX' r : T , 'PROP' () 'LOCAL' () 'SEP' ( SPx ; .. ; SPy ) '|' ( SQx ; .. ; SQy )" :=
   (mk_funspec (pair (cons u%type .. (cons v%type nil) ..) tz) cc_default (atomic_spec_type W T)
    (fun (ts: list Type) => rev_curry (tcurry (fun x1 => .. (tcurry (fun xn => tcurry (fun Q : (T -> mpred) => tcurry (fun (_ : tuple_type tnil) =>
      PROPx (cons Px%type .. (cons Py%type nil) ..)
      (PARAMSx (cons Lx%type .. (cons Ly%type nil) ..) (GLOBALSx (cons Gx .. (cons Gy nil) ..)
-     (SEPx (cons (atomic_shift (fun x => S2) Ei Eo (fun x r => fold_right_sepcon (cons SQx%logic .. (cons SQy%logic nil) ..)) Q) (cons S1x%logic .. (cons S1y%logic nil) ..))))))))) ..)))
+     (SEPx (cons (atomic_shift (fun x => S2) E (fun x r => fold_right_sepcon (cons SQx%logic .. (cons SQy%logic nil) ..)) Q) (cons S1x%logic .. (cons S1y%logic nil) ..))))))))) ..)))
    (fun (ts: list Type) => rev_curry (tcurry (fun x1 => .. (tcurry (fun xn => tcurry (fun Q : (T -> mpred) => tcurry (fun (_ : tuple_type tnil) =>
     @exp (environ -> mpred) _ T (fun r =>
      PROP () (LOCAL () (SEPx (Q r :: cons SPx .. (cons SPy nil) ..)))))))) ..)))
@@ -655,21 +613,20 @@ Notation "'ATOMIC' 'TYPE' W 'OBJ' x 'INVS' Ei Eo 'WITH' x1 , .. , xn 'PRE'  [ u 
       (fun (ts: list Type) => rev_curry (tcurry (fun x1 => .. (tcurry (fun xn (_ : tuple_type tnil) => (cons Lx%type .. (cons Ly%type nil) ..))) ..)))
       (fun (ts: list Type) => rev_curry (tcurry (fun x1 => .. (tcurry (fun xn (_ : tuple_type tnil) => (cons Gx .. (cons Gy nil) ..))) ..)))
       (fun (ts: list Type) => rev_curry (tcurry (fun x1 => .. (tcurry (fun xn (_ : tuple_type tnil) => (cons S1x%logic .. (cons S1y%logic nil) ..))) ..)))
-      (fun (ts: list Type) => rev_curry (tcurry (fun x1 => .. (tcurry (fun xn (_ : tuple_type tnil) x => S2)) ..)))
-      Ei Eo
+      (fun (ts: list Type) => rev_curry (tcurry (fun x1 => .. (tcurry (fun xn (_ : tuple_type tnil) x => S2)) ..))) E
       (fun (ts: list Type) => rev_curry (tcurry (fun x1 => .. (tcurry (fun xn (_ : tuple_type tnil) x r => fold_right_sepcon (cons SQx%logic .. (cons SQy%logic nil) ..))) ..)))
      _ _ _ _ _ _)
   (atomic_spec_nonexpansive_post' W
       (fun (ts: list Type) => rev_curry (tcurry (fun x1 => .. (tcurry (fun xn (_ : tuple_type tnil) r => nil)) ..)))
       (fun (ts: list Type) => rev_curry (tcurry (fun x1 => .. (tcurry (fun xn (_ : tuple_type tnil) r => (cons SPx%assert5%assert3 .. (cons SPy%assert5%assert3 nil) ..))) ..))) _ _))
-  (at level 200, x1 closed binder, xn closed binder, x at level 0, Ei at level 0, Eo at level 0, S2 at level 0, r at level 0, T at level 0).
+  (at level 200, x1 closed binder, xn closed binder, x at level 0, E at level 0, S2 at level 0, r at level 0, T at level 0).
 
-Notation "'ATOMIC' 'TYPE' W 'OBJ' x 'INVS' Ei Eo 'WITH' x1 , .. , xn 'PRE'  [ u , .. , v ] 'PROP' ( Px ; .. ; Py ) 'PARAMS' ( Lx ; .. ; Ly ) 'GLOBALS' ( Gx ; .. ; Gy ) 'SEP' ( S1x ; .. ; S1y ) '|' S2 'POST' [ tz ] 'PROP' () 'LOCAL' ( LQx ; .. ; LQy ) 'SEP' ( SPx ; .. ; SPy ) '|' ( SQx ; .. ; SQy )" :=
+Notation "'ATOMIC' 'TYPE' W 'OBJ' x 'INVS' E 'WITH' x1 , .. , xn 'PRE'  [ u , .. , v ] 'PROP' ( Px ; .. ; Py ) 'PARAMS' ( Lx ; .. ; Ly ) 'GLOBALS' ( Gx ; .. ; Gy ) 'SEP' ( S1x ; .. ; S1y ) '|' S2 'POST' [ tz ] 'PROP' () 'LOCAL' ( LQx ; .. ; LQy ) 'SEP' ( SPx ; .. ; SPy ) '|' ( SQx ; .. ; SQy )" :=
   (mk_funspec (pair (cons u%type .. (cons v%type nil) ..) tz) cc_default (atomic_spec_type0 W)
    (fun (ts: list Type) => rev_curry (tcurry (fun x1 => .. (tcurry (fun xn => tcurry (fun Q : mpred => tcurry (fun (_ : tuple_type tnil) =>
      PROPx (cons Px%type .. (cons Py%type nil) ..)
      (PARAMSx (cons Lx%type .. (cons Ly%type nil) ..) (GLOBALSx (cons Gx .. (cons Gy nil) ..)
-     (SEPx (cons (atomic_shift(B := unit) (fun x => S2) Ei Eo (fun x _ => fold_right_sepcon (cons SQx%logic .. (cons SQy%logic nil) ..)) (fun _ => Q)) (cons S1x%logic .. (cons S1y%logic nil) ..))))))))) ..)))
+     (SEPx (cons (atomic_shift(B := unit) (fun x => S2) (⊤ ∖ E) ∅ (fun x _ => fold_right_sepcon (cons SQx%logic .. (cons SQy%logic nil) ..)) (fun _ => Q)) (cons S1x%logic .. (cons S1y%logic nil) ..))))))))) ..)))
    (fun (ts: list Type) => rev_curry (tcurry (fun x1 => .. (tcurry (fun xn => tcurry (fun Q : mpred => tcurry (fun (_ : tuple_type tnil) =>
      PROP () LOCAL () (SEPx (Q :: cons SPx .. (cons SPy nil) ..)))))) ..)))
    (@atomic_spec_nonexpansive_pre0 _ W
@@ -677,21 +634,20 @@ Notation "'ATOMIC' 'TYPE' W 'OBJ' x 'INVS' Ei Eo 'WITH' x1 , .. , xn 'PRE'  [ u 
       (fun (ts: list Type) => rev_curry (tcurry (fun x1 => .. (tcurry (fun xn (_ : tuple_type tnil) => (cons Lx%type .. (cons Ly%type nil) ..))) ..)))
       (fun (ts: list Type) => rev_curry (tcurry (fun x1 => .. (tcurry (fun xn (_ : tuple_type tnil) => (cons Gx .. (cons Gy nil) ..))) ..)))
       (fun (ts: list Type) => rev_curry (tcurry (fun x1 => .. (tcurry (fun xn (_ : tuple_type tnil) => (cons S1x%logic .. (cons S1y%logic nil) ..))) ..)))
-      (fun (ts: list Type) => rev_curry (tcurry (fun x1 => .. (tcurry (fun xn (_ : tuple_type tnil) x => S2)) ..)))
-      Ei Eo
+      (fun (ts: list Type) => rev_curry (tcurry (fun x1 => .. (tcurry (fun xn (_ : tuple_type tnil) x => S2)) ..))) E
       (fun (ts: list Type) => rev_curry (tcurry (fun x1 => .. (tcurry (fun xn (_ : tuple_type tnil) x _ => fold_right_sepcon (cons SQx%logic .. (cons SQy%logic nil) ..))) ..)))
      _ _ _ _ _ _)
   (atomic_spec_nonexpansive_post0 W
       (fun (ts: list Type) => rev_curry (tcurry (fun x1 => .. (tcurry (fun xn (_ : tuple_type tnil) => (cons LQx%logic .. (cons LQy%logic nil) ..))) ..)))
       (fun (ts: list Type) => rev_curry (tcurry (fun x1 => .. (tcurry (fun xn (_ : tuple_type tnil) => (cons SPx%assert5%assert3 .. (cons SPy%assert5%assert3 nil) ..))) ..))) _ _))
-  (at level 200, x1 closed binder, xn closed binder, x at level 0, Ei at level 0, Eo at level 0, S2 at level 0).
+  (at level 200, x1 closed binder, xn closed binder, x at level 0, E at level 0, S2 at level 0).
 
-Notation "'ATOMIC' 'TYPE' W 'OBJ' x 'INVS' Ei Eo 'WITH' x1 , .. , xn 'PRE'  [ u , .. , v ] 'PROP' ( Px ; .. ; Py ) 'PARAMS' ( Lx ; .. ; Ly ) 'GLOBALS' ( Gx ; .. ; Gy ) 'SEP' ( S1x ; .. ; S1y ) '|' S2 'POST' [ tz ] 'PROP' () 'LOCAL' () 'SEP' ( SPx ; .. ; SPy ) '|' ( SQx ; .. ; SQy )" :=
+Notation "'ATOMIC' 'TYPE' W 'OBJ' x 'INVS' E 'WITH' x1 , .. , xn 'PRE'  [ u , .. , v ] 'PROP' ( Px ; .. ; Py ) 'PARAMS' ( Lx ; .. ; Ly ) 'GLOBALS' ( Gx ; .. ; Gy ) 'SEP' ( S1x ; .. ; S1y ) '|' S2 'POST' [ tz ] 'PROP' () 'LOCAL' () 'SEP' ( SPx ; .. ; SPy ) '|' ( SQx ; .. ; SQy )" :=
   (mk_funspec (pair (cons u%type .. (cons v%type nil) ..) tz) cc_default (atomic_spec_type0 W)
    (fun (ts: list Type) => rev_curry (tcurry (fun x1 => .. (tcurry (fun xn => tcurry (fun Q : mpred => tcurry (fun (_ : tuple_type tnil) =>
      PROPx (cons Px%type .. (cons Py%type nil) ..)
      (PARAMSx (cons Lx%type .. (cons Ly%type nil) ..) (GLOBALSx (cons Gx .. (cons Gy nil) ..)
-     (SEPx (cons (atomic_shift(B := unit) (fun x => S2) Ei Eo (fun x _ => fold_right_sepcon (cons SQx%logic .. (cons SQy%logic nil) ..)) (fun _ => Q)) (cons S1x%logic .. (cons S1y%logic nil) ..))))))))) ..)))
+     (SEPx (cons (atomic_shift(B := unit) (fun x => S2) (⊤ ∖ E) ∅ (fun x _ => fold_right_sepcon (cons SQx%logic .. (cons SQy%logic nil) ..)) (fun _ => Q)) (cons S1x%logic .. (cons S1y%logic nil) ..))))))))) ..)))
    (fun (ts: list Type) => rev_curry (tcurry (fun x1 => .. (tcurry (fun xn => tcurry (fun Q : mpred => tcurry (fun (_ : tuple_type tnil) =>
      PROP () LOCAL () (SEPx (Q :: cons SPx .. (cons SPy nil) ..)))))) ..)))
    (@atomic_spec_nonexpansive_pre0 _ W
@@ -699,21 +655,20 @@ Notation "'ATOMIC' 'TYPE' W 'OBJ' x 'INVS' Ei Eo 'WITH' x1 , .. , xn 'PRE'  [ u 
       (fun (ts: list Type) => rev_curry (tcurry (fun x1 => .. (tcurry (fun xn (_ : tuple_type tnil) => (cons Lx%type .. (cons Ly%type nil) ..))) ..)))
       (fun (ts: list Type) => rev_curry (tcurry (fun x1 => .. (tcurry (fun xn (_ : tuple_type tnil) => (cons Gx .. (cons Gy nil) ..))) ..)))
       (fun (ts: list Type) => rev_curry (tcurry (fun x1 => .. (tcurry (fun xn (_ : tuple_type tnil) => (cons S1x%logic .. (cons S1y%logic nil) ..))) ..)))
-      (fun (ts: list Type) => rev_curry (tcurry (fun x1 => .. (tcurry (fun xn (_ : tuple_type tnil) x => S2)) ..)))
-      Ei Eo
+      (fun (ts: list Type) => rev_curry (tcurry (fun x1 => .. (tcurry (fun xn (_ : tuple_type tnil) x => S2)) ..))) E
       (fun (ts: list Type) => rev_curry (tcurry (fun x1 => .. (tcurry (fun xn (_ : tuple_type tnil) x _ => fold_right_sepcon (cons SQx%logic .. (cons SQy%logic nil) ..))) ..)))
      _ _ _ _ _ _)
   (atomic_spec_nonexpansive_post0 W
       (fun (ts: list Type) => rev_curry (tcurry (fun x1 => .. (tcurry (fun xn (_ : tuple_type tnil) => nil)) ..)))
       (fun (ts: list Type) => rev_curry (tcurry (fun x1 => .. (tcurry (fun xn (_ : tuple_type tnil) => (cons SPx%assert5%assert3 .. (cons SPy%assert5%assert3 nil) ..))) ..))) _ _))
-  (at level 200, x1 closed binder, xn closed binder, x at level 0, Ei at level 0, Eo at level 0, S2 at level 0).
+  (at level 200, x1 closed binder, xn closed binder, x at level 0, E at level 0, S2 at level 0).
 
-Notation "'ATOMIC' 'TYPE' W 'OBJ' x 'INVS' Ei Eo 'WITH' x1 , .. , xn 'PRE'  [ ] 'PROP' ( Px ; .. ; Py ) 'PARAMS' ( Lx ; .. ; Ly ) 'GLOBALS' ( Gx ; .. ; Gy ) 'SEP' ( S1x ; .. ; S1y ) '|' S2 'POST' [ tz ] 'EX' r : T , 'PROP' () 'LOCAL' ( LQx ; .. ; LQy ) 'SEP' ( SPx ; .. ; SPy ) '|' ( SQx ; .. ; SQy )" :=
+Notation "'ATOMIC' 'TYPE' W 'OBJ' x 'INVS' E 'WITH' x1 , .. , xn 'PRE'  [ ] 'PROP' ( Px ; .. ; Py ) 'PARAMS' ( Lx ; .. ; Ly ) 'GLOBALS' ( Gx ; .. ; Gy ) 'SEP' ( S1x ; .. ; S1y ) '|' S2 'POST' [ tz ] 'EX' r : T , 'PROP' () 'LOCAL' ( LQx ; .. ; LQy ) 'SEP' ( SPx ; .. ; SPy ) '|' ( SQx ; .. ; SQy )" :=
   (mk_funspec (pair nil tz) cc_default (atomic_spec_type W T)
    (fun (ts: list Type) => rev_curry (tcurry (fun x1 => .. (tcurry (fun xn => tcurry (fun Q : (T -> mpred) => tcurry (fun (_ : tuple_type tnil) =>
      PROPx (cons Px%type .. (cons Py%type nil) ..)
      (PARAMSx (cons Lx%type .. (cons Ly%type nil) ..) (GLOBALSx (cons Gx .. (cons Gy nil) ..)
-     (SEPx (cons (atomic_shift (fun x => S2) Ei Eo (fun x r => fold_right_sepcon (cons SQx%logic .. (cons SQy%logic nil) ..)) Q) (cons S1x%logic .. (cons S1y%logic nil) ..))))))))) ..)))
+     (SEPx (cons (atomic_shift (fun x => S2) (⊤ ∖ E) ∅ (fun x r => fold_right_sepcon (cons SQx%logic .. (cons SQy%logic nil) ..)) Q) (cons S1x%logic .. (cons S1y%logic nil) ..))))))))) ..)))
    (fun (ts: list Type) => rev_curry (tcurry (fun x1 => .. (tcurry (fun xn => tcurry (fun Q : (T -> mpred) => tcurry (fun (_ : tuple_type tnil) =>
     @exp (environ -> mpred) _ T (fun r =>
      PROP () (LOCALx (cons LQx .. (cons LQy nil) ..) ((SEPx (Q r :: cons SPx .. (cons SPy nil) ..))))))))) ..)))
@@ -722,21 +677,20 @@ Notation "'ATOMIC' 'TYPE' W 'OBJ' x 'INVS' Ei Eo 'WITH' x1 , .. , xn 'PRE'  [ ] 
       (fun (ts: list Type) => rev_curry (tcurry (fun x1 => .. (tcurry (fun xn (_ : tuple_type tnil) => (cons Lx%type .. (cons Ly%type nil) ..))) ..)))
       (fun (ts: list Type) => rev_curry (tcurry (fun x1 => .. (tcurry (fun xn (_ : tuple_type tnil) => (cons Gx .. (cons Gy nil) ..))) ..)))
       (fun (ts: list Type) => rev_curry (tcurry (fun x1 => .. (tcurry (fun xn (_ : tuple_type tnil) => (cons S1x%logic .. (cons S1y%logic nil) ..))) ..)))
-      (fun (ts: list Type) => rev_curry (tcurry (fun x1 => .. (tcurry (fun xn (_ : tuple_type tnil) x => S2)) ..)))
-      Ei Eo
+      (fun (ts: list Type) => rev_curry (tcurry (fun x1 => .. (tcurry (fun xn (_ : tuple_type tnil) x => S2)) ..))) E
       (fun (ts: list Type) => rev_curry (tcurry (fun x1 => .. (tcurry (fun xn (_ : tuple_type tnil) x r => fold_right_sepcon (cons SQx%logic .. (cons SQy%logic nil) ..))) ..)))
      _ _ _ _ _ _)
   (atomic_spec_nonexpansive_post' W
       (fun (ts: list Type) => rev_curry (tcurry (fun x1 => .. (tcurry (fun xn (_ : tuple_type tnil) r => (cons LQx%assert3 .. (cons LQy%assert3 nil) ..))) ..)))
       (fun (ts: list Type) => rev_curry (tcurry (fun x1 => .. (tcurry (fun xn (_ : tuple_type tnil) r => (cons SPx%assert3 .. (cons SPy%assert3 nil) ..))) ..))) _ _))
-  (at level 200, x1 closed binder, xn closed binder, x at level 0, Ei at level 0, Eo at level 0, S2 at level 0, r at level 0, T at level 0).
+  (at level 200, x1 closed binder, xn closed binder, x at level 0, E at level 0, S2 at level 0, r at level 0, T at level 0).
 
-Notation "'ATOMIC' 'TYPE' W 'OBJ' x 'INVS' Ei Eo 'WITH' x1 , .. , xn 'PRE'  [ ] 'PROP' ( Px ; .. ; Py ) 'PARAMS' ( Lx ; .. ; Ly ) 'GLOBALS' ( Gx ; .. ; Gy ) 'SEP' ( S1x ; .. ; S1y ) '|' S2 'POST' [ tz ] 'EX' r : T , 'PROP' () 'LOCAL' () 'SEP' ( SPx ; .. ; SPy ) '|' ( SQx ; .. ; SQy )" :=
+Notation "'ATOMIC' 'TYPE' W 'OBJ' x 'INVS' E 'WITH' x1 , .. , xn 'PRE'  [ ] 'PROP' ( Px ; .. ; Py ) 'PARAMS' ( Lx ; .. ; Ly ) 'GLOBALS' ( Gx ; .. ; Gy ) 'SEP' ( S1x ; .. ; S1y ) '|' S2 'POST' [ tz ] 'EX' r : T , 'PROP' () 'LOCAL' () 'SEP' ( SPx ; .. ; SPy ) '|' ( SQx ; .. ; SQy )" :=
   (mk_funspec (pair nil tz) cc_default (atomic_spec_type W T)
    (fun (ts: list Type) => rev_curry (tcurry (fun x1 => .. (tcurry (fun xn => tcurry (fun Q : (T -> mpred) => tcurry (fun (_ : tuple_type tnil) =>
      PROPx (cons Px%type .. (cons Py%type nil) ..)
      (PARAMSx (cons Lx%type .. (cons Ly%type nil) ..) (GLOBALSx (cons Gx .. (cons Gy nil) ..)
-     (SEPx (cons (atomic_shift (fun x => S2) Ei Eo (fun x r => fold_right_sepcon (cons SQx%logic .. (cons SQy%logic nil) ..)) Q) (cons S1x%logic .. (cons S1y%logic nil) ..))))))))) ..)))
+     (SEPx (cons (atomic_shift (fun x => S2) (⊤ ∖ E) ∅ (fun x r => fold_right_sepcon (cons SQx%logic .. (cons SQy%logic nil) ..)) Q) (cons S1x%logic .. (cons S1y%logic nil) ..))))))))) ..)))
    (fun (ts: list Type) => rev_curry (tcurry (fun x1 => .. (tcurry (fun xn => tcurry (fun Q : (T -> mpred) => tcurry (fun (_ : tuple_type tnil) =>
     @exp (environ -> mpred) _ T (fun r =>
      PROP () (LOCAL () (SEPx (Q r :: cons SPx .. (cons SPy nil) ..)))))))) ..)))
@@ -745,21 +699,20 @@ Notation "'ATOMIC' 'TYPE' W 'OBJ' x 'INVS' Ei Eo 'WITH' x1 , .. , xn 'PRE'  [ ] 
       (fun (ts: list Type) => rev_curry (tcurry (fun x1 => .. (tcurry (fun xn (_ : tuple_type tnil) => (cons Lx%type .. (cons Ly%type nil) ..))) ..)))
       (fun (ts: list Type) => rev_curry (tcurry (fun x1 => .. (tcurry (fun xn (_ : tuple_type tnil) => (cons Gx .. (cons Gy nil) ..))) ..)))
       (fun (ts: list Type) => rev_curry (tcurry (fun x1 => .. (tcurry (fun xn (_ : tuple_type tnil) => (cons S1x%logic .. (cons S1y%logic nil) ..))) ..)))
-      (fun (ts: list Type) => rev_curry (tcurry (fun x1 => .. (tcurry (fun xn (_ : tuple_type tnil) x => S2)) ..)))
-      Ei Eo
+      (fun (ts: list Type) => rev_curry (tcurry (fun x1 => .. (tcurry (fun xn (_ : tuple_type tnil) x => S2)) ..))) E
       (fun (ts: list Type) => rev_curry (tcurry (fun x1 => .. (tcurry (fun xn (_ : tuple_type tnil) x r => fold_right_sepcon (cons SQx%logic .. (cons SQy%logic nil) ..))) ..)))
      _ _ _ _ _ _)
   (atomic_spec_nonexpansive_post' W
       (fun (ts: list Type) => rev_curry (tcurry (fun x1 => .. (tcurry (fun xn (_ : tuple_type tnil) r => nil)) ..)))
       (fun (ts: list Type) => rev_curry (tcurry (fun x1 => .. (tcurry (fun xn (_ : tuple_type tnil) r => (cons SPx%assert5%assert3 .. (cons SPy%assert5%assert3 nil) ..))) ..))) _ _))
-  (at level 200, x1 closed binder, xn closed binder, x at level 0, Ei at level 0, Eo at level 0, S2 at level 0, r at level 0, T at level 0).
+  (at level 200, x1 closed binder, xn closed binder, x at level 0, E at level 0, S2 at level 0, r at level 0, T at level 0).
 
-Notation "'ATOMIC' 'TYPE' W 'OBJ' x 'INVS' Ei Eo 'WITH' x1 , .. , xn 'PRE'  [ ] 'PROP' ( Px ; .. ; Py ) 'PARAMS ( Lx ; .. ; Ly ) 'GLOBALS' ( Gx ; .. ; Gy ) 'SEP' ( S1x ; .. ; S1y ) '|' S2 'POST' [ tz ] 'PROP' () 'LOCAL' ( LQx ; .. ; LQy ) 'SEP' ( SPx ; .. ; SPy ) '|' ( SQx ; .. ; SQy )" :=
+Notation "'ATOMIC' 'TYPE' W 'OBJ' x 'INVS' E 'WITH' x1 , .. , xn 'PRE'  [ ] 'PROP' ( Px ; .. ; Py ) 'PARAMS ( Lx ; .. ; Ly ) 'GLOBALS' ( Gx ; .. ; Gy ) 'SEP' ( S1x ; .. ; S1y ) '|' S2 'POST' [ tz ] 'PROP' () 'LOCAL' ( LQx ; .. ; LQy ) 'SEP' ( SPx ; .. ; SPy ) '|' ( SQx ; .. ; SQy )" :=
   (mk_funspec (pair nil tz) cc_default (atomic_spec_type0 W)
    (fun (ts: list Type) => rev_curry (tcurry (fun x1 => .. (tcurry (fun xn => tcurry (fun Q : mpred => tcurry (fun (_ : tuple_type tnil) =>
      PROPx (cons Px%type .. (cons Py%type nil) ..)
      (PARAMSx (cons Lx%type .. (cons Ly%type nil) ..) (GLOBALSx (cons Gx .. (cons Gy nil) ..)
-     (SEPx (cons (atomic_shift(B := unit) (fun x => S2) Ei Eo (fun x _ => fold_right_sepcon (cons SQx%logic .. (cons SQy%logic nil) ..)) (fun _ => Q)) (cons S1x%logic .. (cons S1y%logic nil) ..))))))))) ..)))
+     (SEPx (cons (atomic_shift(B := unit) (fun x => S2) (⊤ ∖ E) ∅ (fun x _ => fold_right_sepcon (cons SQx%logic .. (cons SQy%logic nil) ..)) (fun _ => Q)) (cons S1x%logic .. (cons S1y%logic nil) ..))))))))) ..)))
    (fun (ts: list Type) => rev_curry (tcurry (fun x1 => .. (tcurry (fun xn => tcurry (fun Q : mpred => tcurry (fun (_ : tuple_type tnil) =>
      PROP () LOCAL () (SEPx (Q :: cons SPx .. (cons SPy nil) ..)))))) ..)))
    (@atomic_spec_nonexpansive_pre0 _ W
@@ -767,21 +720,20 @@ Notation "'ATOMIC' 'TYPE' W 'OBJ' x 'INVS' Ei Eo 'WITH' x1 , .. , xn 'PRE'  [ ] 
       (fun (ts: list Type) => rev_curry (tcurry (fun x1 => .. (tcurry (fun xn (_ : tuple_type tnil) => (cons Lx%type .. (cons Ly%type nil) ..))) ..)))
       (fun (ts: list Type) => rev_curry (tcurry (fun x1 => .. (tcurry (fun xn (_ : tuple_type tnil) => (cons Gx .. (cons Gy nil) ..))) ..)))
       (fun (ts: list Type) => rev_curry (tcurry (fun x1 => .. (tcurry (fun xn (_ : tuple_type tnil) => (cons S1x%logic .. (cons S1y%logic nil) ..))) ..)))
-      (fun (ts: list Type) => rev_curry (tcurry (fun x1 => .. (tcurry (fun xn (_ : tuple_type tnil) x => S2)) ..)))
-      Ei Eo
+      (fun (ts: list Type) => rev_curry (tcurry (fun x1 => .. (tcurry (fun xn (_ : tuple_type tnil) x => S2)) ..))) E
       (fun (ts: list Type) => rev_curry (tcurry (fun x1 => .. (tcurry (fun xn (_ : tuple_type tnil) x _ => fold_right_sepcon (cons SQx%logic .. (cons SQy%logic nil) ..))) ..)))
      _ _ _ _ _ _)
   (atomic_spec_nonexpansive_post0 W
       (fun (ts: list Type) => rev_curry (tcurry (fun x1 => .. (tcurry (fun xn (_ : tuple_type tnil) => (cons LQx%logic .. (cons LQy%logic nil) ..))) ..)))
       (fun (ts: list Type) => rev_curry (tcurry (fun x1 => .. (tcurry (fun xn (_ : tuple_type tnil) => (cons SPx%assert5%assert3 .. (cons SPy%assert5%assert3 nil) ..))) ..))) _ _))
-  (at level 200, x1 closed binder, xn closed binder, x at level 0, Ei at level 0, Eo at level 0, S2 at level 0).
+  (at level 200, x1 closed binder, xn closed binder, x at level 0, E at level 0, S2 at level 0).
 
-Notation "'ATOMIC' 'TYPE' W 'OBJ' x 'INVS' Ei Eo 'WITH' x1 , .. , xn 'PRE'  [ ] 'PROP' ( Px ; .. ; Py ) 'PARAMS' ( Lx ; .. ; Ly ) 'GLOBALS' ( Gx ; .. ; Gy ) 'SEP' ( S1x ; .. ; S1y ) '|' S2 'POST' [ tz ] 'PROP' () 'LOCAL' () 'SEP' ( SPx ; .. ; SPy ) '|' ( SQx ; .. ; SQy )" :=
+Notation "'ATOMIC' 'TYPE' W 'OBJ' x 'INVS' E 'WITH' x1 , .. , xn 'PRE'  [ ] 'PROP' ( Px ; .. ; Py ) 'PARAMS' ( Lx ; .. ; Ly ) 'GLOBALS' ( Gx ; .. ; Gy ) 'SEP' ( S1x ; .. ; S1y ) '|' S2 'POST' [ tz ] 'PROP' () 'LOCAL' () 'SEP' ( SPx ; .. ; SPy ) '|' ( SQx ; .. ; SQy )" :=
   (mk_funspec (pair nil tz) cc_default (atomic_spec_type0 W)
    (fun (ts: list Type) => rev_curry (tcurry (fun x1 => .. (tcurry (fun xn => tcurry (fun Q : mpred => tcurry (fun (_ : tuple_type tnil) =>
      PROPx (cons Px%type .. (cons Py%type nil) ..)
      (PARAMSx (cons Lx%type .. (cons Ly%type nil) ..) (GLOBALSx (cons Gx .. (cons Gy nil) ..)
-     (SEPx (cons (atomic_shift(B := unit) (fun x => S2) Ei Eo (fun x _ => fold_right_sepcon (cons SQx%logic .. (cons SQy%logic nil) ..)) (fun _ => Q)) (cons S1x%logic .. (cons S1y%logic nil) ..))))))))) ..)))
+     (SEPx (cons (atomic_shift(B := unit) (fun x => S2) (⊤ ∖ E) ∅ (fun x _ => fold_right_sepcon (cons SQx%logic .. (cons SQy%logic nil) ..)) (fun _ => Q)) (cons S1x%logic .. (cons S1y%logic nil) ..))))))))) ..)))
    (fun (ts: list Type) => rev_curry (tcurry (fun x1 => .. (tcurry (fun xn => tcurry (fun Q : mpred => tcurry (fun (_ : tuple_type tnil) =>
      PROP () LOCAL () (SEPx (Q :: cons SPx .. (cons SPy nil) ..)))))) ..)))
    (@atomic_spec_nonexpansive_pre0 _ W
@@ -789,21 +741,20 @@ Notation "'ATOMIC' 'TYPE' W 'OBJ' x 'INVS' Ei Eo 'WITH' x1 , .. , xn 'PRE'  [ ] 
       (fun (ts: list Type) => rev_curry (tcurry (fun x1 => .. (tcurry (fun xn (_ : tuple_type tnil) => (cons Lx%type .. (cons Ly%type nil) ..))) ..)))
       (fun (ts: list Type) => rev_curry (tcurry (fun x1 => .. (tcurry (fun xn (_ : tuple_type tnil) => (cons Gx .. (cons Gy nil) ..))) ..)))
       (fun (ts: list Type) => rev_curry (tcurry (fun x1 => .. (tcurry (fun xn (_ : tuple_type tnil) => (cons S1x%logic .. (cons S1y%logic nil) ..))) ..)))
-      (fun (ts: list Type) => rev_curry (tcurry (fun x1 => .. (tcurry (fun xn (_ : tuple_type tnil) x => S2)) ..)))
-      Ei Eo
+      (fun (ts: list Type) => rev_curry (tcurry (fun x1 => .. (tcurry (fun xn (_ : tuple_type tnil) x => S2)) ..))) E
       (fun (ts: list Type) => rev_curry (tcurry (fun x1 => .. (tcurry (fun xn (_ : tuple_type tnil) x _ => fold_right_sepcon (cons SQx%logic .. (cons SQy%logic nil) ..))) ..)))
      _ _ _ _ _ _)
   (atomic_spec_nonexpansive_post0 W
       (fun (ts: list Type) => rev_curry (tcurry (fun x1 => .. (tcurry (fun xn (_ : tuple_type tnil) => nil)) ..)))
       (fun (ts: list Type) => rev_curry (tcurry (fun x1 => .. (tcurry (fun xn (_ : tuple_type tnil) => (cons SPx%assert5%assert3 .. (cons SPy%assert5%assert3 nil) ..))) ..))) _ _))
-  (at level 200, x1 closed binder, xn closed binder, x at level 0, Ei at level 0, Eo at level 0, S2 at level 0).
+  (at level 200, x1 closed binder, xn closed binder, x at level 0, E at level 0, S2 at level 0).
 
-Notation "'ATOMIC' 'TYPE' W 'OBJ' x 'INVS' Ei Eo 'WITH' x1 , .. , xn 'PRE'  [ u , .. , v ] 'PROP' ( Px ; .. ; Py ) 'PARAMS' () 'GLOBALS' ( Gx ; .. ; Gy ) 'SEP' ( S1x ; .. ; S1y ) '|' S2 'POST' [ tz ] 'EX' r : T , 'PROP' () 'LOCAL' ( LQx ; .. ; LQy ) 'SEP' ( SPx ; .. ; SPy ) '|' ( SQx ; .. ; SQy )" :=
+Notation "'ATOMIC' 'TYPE' W 'OBJ' x 'INVS' E 'WITH' x1 , .. , xn 'PRE'  [ u , .. , v ] 'PROP' ( Px ; .. ; Py ) 'PARAMS' () 'GLOBALS' ( Gx ; .. ; Gy ) 'SEP' ( S1x ; .. ; S1y ) '|' S2 'POST' [ tz ] 'EX' r : T , 'PROP' () 'LOCAL' ( LQx ; .. ; LQy ) 'SEP' ( SPx ; .. ; SPy ) '|' ( SQx ; .. ; SQy )" :=
   (mk_funspec (pair (cons u%type .. (cons v%type nil) ..) tz) cc_default (atomic_spec_type W T)
    (fun (ts: list Type) => rev_curry (tcurry (fun x1 => .. (tcurry (fun xn => tcurry (fun Q : (T -> mpred) => tcurry (fun (_ : tuple_type tnil) =>
      PROPx (cons Px%type .. (cons Py%type nil) ..)
      (PARAMSx nil (GLOBALSx (cons Gx .. (cons Gy nil) ..)
-     (SEPx (cons (atomic_shift (fun x => S2) Ei Eo (fun x r => fold_right_sepcon (cons SQx%logic .. (cons SQy%logic nil) ..)) Q) (cons S1x%logic .. (cons S1y%logic nil) ..))))))))) ..)))
+     (SEPx (cons (atomic_shift (fun x => S2) (⊤ ∖ E) ∅ (fun x r => fold_right_sepcon (cons SQx%logic .. (cons SQy%logic nil) ..)) Q) (cons S1x%logic .. (cons S1y%logic nil) ..))))))))) ..)))
    (fun (ts: list Type) => rev_curry (tcurry (fun x1 => .. (tcurry (fun xn => tcurry (fun Q : (T -> mpred) => tcurry (fun (_ : tuple_type tnil) =>
     @exp (environ -> mpred) _ T (fun r =>
      PROP () (LOCALx (cons LQx .. (cons LQy nil) ..) ((SEPx (Q r :: cons SPx .. (cons SPy nil) ..))))))))) ..)))
@@ -812,21 +763,20 @@ Notation "'ATOMIC' 'TYPE' W 'OBJ' x 'INVS' Ei Eo 'WITH' x1 , .. , xn 'PRE'  [ u 
       (fun (ts: list Type) => rev_curry (tcurry (fun x1 => .. (tcurry (fun xn (_ : tuple_type tnil) => nil)) ..)))
       (fun (ts: list Type) => rev_curry (tcurry (fun x1 => .. (tcurry (fun xn (_ : tuple_type tnil) => (cons Gx .. (cons Gy nil) ..))) ..)))
       (fun (ts: list Type) => rev_curry (tcurry (fun x1 => .. (tcurry (fun xn (_ : tuple_type tnil) => (cons S1x%logic .. (cons S1y%logic nil) ..))) ..)))
-      (fun (ts: list Type) => rev_curry (tcurry (fun x1 => .. (tcurry (fun xn (_ : tuple_type tnil) x => S2)) ..)))
-      Ei Eo
+      (fun (ts: list Type) => rev_curry (tcurry (fun x1 => .. (tcurry (fun xn (_ : tuple_type tnil) x => S2)) ..))) E
       (fun (ts: list Type) => rev_curry (tcurry (fun x1 => .. (tcurry (fun xn (_ : tuple_type tnil) x r => fold_right_sepcon (cons SQx%logic .. (cons SQy%logic nil) ..))) ..)))
      _ _ _ _ _ _)
   (atomic_spec_nonexpansive_post' W
       (fun (ts: list Type) => rev_curry (tcurry (fun x1 => .. (tcurry (fun xn (_ : tuple_type tnil) r => (cons LQx%assert3 .. (cons LQy%assert3 nil) ..))) ..)))
       (fun (ts: list Type) => rev_curry (tcurry (fun x1 => .. (tcurry (fun xn (_ : tuple_type tnil) r => (cons SPx%assert3 .. (cons SPy%assert3 nil) ..))) ..))) _ _))
-  (at level 200, x1 closed binder, xn closed binder, x at level 0, Ei at level 0, Eo at level 0, S2 at level 0, r at level 0, T at level 0).
+  (at level 200, x1 closed binder, xn closed binder, x at level 0, E at level 0, S2 at level 0, r at level 0, T at level 0).
 
-Notation "'ATOMIC' 'TYPE' W 'OBJ' x 'INVS' Ei Eo 'WITH' x1 , .. , xn 'PRE'  [ u , .. , v ] 'PROP' ( Px ; .. ; Py ) 'PARAMS' () 'GLOBALS' ( Gx ; .. ; Gy ) 'SEP' ( S1x ; .. ; S1y ) '|' S2 'POST' [ tz ] 'EX' r : T , 'PROP' () 'LOCAL' () 'SEP' ( SPx ; .. ; SPy ) '|' ( SQx ; .. ; SQy )" :=
+Notation "'ATOMIC' 'TYPE' W 'OBJ' x 'INVS' E 'WITH' x1 , .. , xn 'PRE'  [ u , .. , v ] 'PROP' ( Px ; .. ; Py ) 'PARAMS' () 'GLOBALS' ( Gx ; .. ; Gy ) 'SEP' ( S1x ; .. ; S1y ) '|' S2 'POST' [ tz ] 'EX' r : T , 'PROP' () 'LOCAL' () 'SEP' ( SPx ; .. ; SPy ) '|' ( SQx ; .. ; SQy )" :=
   (mk_funspec (pair (cons u%type .. (cons v%type nil) ..) tz) cc_default (atomic_spec_type W T)
    (fun (ts: list Type) => rev_curry (tcurry (fun x1 => .. (tcurry (fun xn => tcurry (fun Q : (T -> mpred) => tcurry (fun (_ : tuple_type tnil) =>
      PROPx (cons Px%type .. (cons Py%type nil) ..)
      (PARAMSx nil (GLOBALSx (cons Gx .. (cons Gy nil) ..)
-     (SEPx (cons (atomic_shift (fun x => S2) Ei Eo (fun x r => fold_right_sepcon (cons SQx%logic .. (cons SQy%logic nil) ..)) Q) (cons S1x%logic .. (cons S1y%logic nil) ..))))))))) ..)))
+     (SEPx (cons (atomic_shift (fun x => S2) (⊤ ∖ E) ∅ (fun x r => fold_right_sepcon (cons SQx%logic .. (cons SQy%logic nil) ..)) Q) (cons S1x%logic .. (cons S1y%logic nil) ..))))))))) ..)))
    (fun (ts: list Type) => rev_curry (tcurry (fun x1 => .. (tcurry (fun xn => tcurry (fun Q : (T -> mpred) => tcurry (fun (_ : tuple_type tnil) =>
     @exp (environ -> mpred) _ T (fun r =>
      PROP () (LOCAL () (SEPx (Q r :: cons SPx .. (cons SPy nil) ..)))))))) ..)))
@@ -835,21 +785,20 @@ Notation "'ATOMIC' 'TYPE' W 'OBJ' x 'INVS' Ei Eo 'WITH' x1 , .. , xn 'PRE'  [ u 
       (fun (ts: list Type) => rev_curry (tcurry (fun x1 => .. (tcurry (fun xn (_ : tuple_type tnil) => nil)) ..)))
       (fun (ts: list Type) => rev_curry (tcurry (fun x1 => .. (tcurry (fun xn (_ : tuple_type tnil) => (cons Gx .. (cons Gy nil) ..))) ..)))
       (fun (ts: list Type) => rev_curry (tcurry (fun x1 => .. (tcurry (fun xn (_ : tuple_type tnil) => (cons S1x%logic .. (cons S1y%logic nil) ..))) ..)))
-      (fun (ts: list Type) => rev_curry (tcurry (fun x1 => .. (tcurry (fun xn (_ : tuple_type tnil) x => S2)) ..)))
-      Ei Eo
+      (fun (ts: list Type) => rev_curry (tcurry (fun x1 => .. (tcurry (fun xn (_ : tuple_type tnil) x => S2)) ..))) E
       (fun (ts: list Type) => rev_curry (tcurry (fun x1 => .. (tcurry (fun xn (_ : tuple_type tnil) x r => fold_right_sepcon (cons SQx%logic .. (cons SQy%logic nil) ..))) ..)))
      _ _ _ _ _ _)
   (atomic_spec_nonexpansive_post' W
       (fun (ts: list Type) => rev_curry (tcurry (fun x1 => .. (tcurry (fun xn (_ : tuple_type tnil) r => nil)) ..)))
       (fun (ts: list Type) => rev_curry (tcurry (fun x1 => .. (tcurry (fun xn (_ : tuple_type tnil) r => (cons SPx%assert5%assert3 .. (cons SPy%assert5%assert3 nil) ..))) ..))) _ _))
-  (at level 200, x1 closed binder, xn closed binder, x at level 0, Ei at level 0, Eo at level 0, S2 at level 0, r at level 0, T at level 0).
+  (at level 200, x1 closed binder, xn closed binder, x at level 0, E at level 0, S2 at level 0, r at level 0, T at level 0).
 
-Notation "'ATOMIC' 'TYPE' W 'OBJ' x 'INVS' Ei Eo 'WITH' x1 , .. , xn 'PRE'  [ u , .. , v ] 'PROP' ( Px ; .. ; Py ) 'PARAMS' () 'GLOBALS' ( Gx ; .. ; Gy ) 'SEP' ( S1x ; .. ; S1y ) '|' S2 'POST' [ tz ] 'PROP' () 'LOCAL' ( LQx ; .. ; LQy ) 'SEP' ( SPx ; .. ; SPy ) '|' ( SQx ; .. ; SQy )" :=
+Notation "'ATOMIC' 'TYPE' W 'OBJ' x 'INVS' E 'WITH' x1 , .. , xn 'PRE'  [ u , .. , v ] 'PROP' ( Px ; .. ; Py ) 'PARAMS' () 'GLOBALS' ( Gx ; .. ; Gy ) 'SEP' ( S1x ; .. ; S1y ) '|' S2 'POST' [ tz ] 'PROP' () 'LOCAL' ( LQx ; .. ; LQy ) 'SEP' ( SPx ; .. ; SPy ) '|' ( SQx ; .. ; SQy )" :=
   (mk_funspec (pair (cons u%type .. (cons v%type nil) ..) tz) cc_default (atomic_spec_type0 W)
    (fun (ts: list Type) => rev_curry (tcurry (fun x1 => .. (tcurry (fun xn => tcurry (fun Q : mpred => tcurry (fun (_ : tuple_type tnil) =>
      PROPx (cons Px%type .. (cons Py%type nil) ..)
      (PARAMSx nil (GLOBALSx (cons Gx .. (cons Gy nil) ..)
-     (SEPx (cons (atomic_shift(B := unit) (fun x => S2) Ei Eo (fun x _ => fold_right_sepcon (cons SQx%logic .. (cons SQy%logic nil) ..)) (fun _ => Q)) (cons S1x%logic .. (cons S1y%logic nil) ..))))))))) ..)))
+     (SEPx (cons (atomic_shift(B := unit) (fun x => S2) (⊤ ∖ E) ∅ (fun x _ => fold_right_sepcon (cons SQx%logic .. (cons SQy%logic nil) ..)) (fun _ => Q)) (cons S1x%logic .. (cons S1y%logic nil) ..))))))))) ..)))
    (fun (ts: list Type) => rev_curry (tcurry (fun x1 => .. (tcurry (fun xn => tcurry (fun Q : mpred => tcurry (fun (_ : tuple_type tnil) =>
      PROP () LOCAL () (SEPx (Q :: cons SPx .. (cons SPy nil) ..)))))) ..)))
    (@atomic_spec_nonexpansive_pre0 _ W
@@ -857,21 +806,20 @@ Notation "'ATOMIC' 'TYPE' W 'OBJ' x 'INVS' Ei Eo 'WITH' x1 , .. , xn 'PRE'  [ u 
       (fun (ts: list Type) => rev_curry (tcurry (fun x1 => .. (tcurry (fun xn (_ : tuple_type tnil) => nil)) ..)))
       (fun (ts: list Type) => rev_curry (tcurry (fun x1 => .. (tcurry (fun xn (_ : tuple_type tnil) => (cons Gx .. (cons Gy nil) ..))) ..)))
       (fun (ts: list Type) => rev_curry (tcurry (fun x1 => .. (tcurry (fun xn (_ : tuple_type tnil) => (cons S1x%logic .. (cons S1y%logic nil) ..))) ..)))
-      (fun (ts: list Type) => rev_curry (tcurry (fun x1 => .. (tcurry (fun xn (_ : tuple_type tnil) x => S2)) ..)))
-      Ei Eo
+      (fun (ts: list Type) => rev_curry (tcurry (fun x1 => .. (tcurry (fun xn (_ : tuple_type tnil) x => S2)) ..))) E
       (fun (ts: list Type) => rev_curry (tcurry (fun x1 => .. (tcurry (fun xn (_ : tuple_type tnil) x _ => fold_right_sepcon (cons SQx%logic .. (cons SQy%logic nil) ..))) ..)))
      _ _ _ _ _ _)
   (atomic_spec_nonexpansive_post0 W
       (fun (ts: list Type) => rev_curry (tcurry (fun x1 => .. (tcurry (fun xn (_ : tuple_type tnil) => (cons LQx%logic .. (cons LQy%logic nil) ..))) ..)))
       (fun (ts: list Type) => rev_curry (tcurry (fun x1 => .. (tcurry (fun xn (_ : tuple_type tnil) => (cons SPx%assert5%assert3 .. (cons SPy%assert5%assert3 nil) ..))) ..))) _ _))
-  (at level 200, x1 closed binder, xn closed binder, x at level 0, Ei at level 0, Eo at level 0, S2 at level 0).
+  (at level 200, x1 closed binder, xn closed binder, x at level 0, E at level 0, S2 at level 0).
 
-Notation "'ATOMIC' 'TYPE' W 'OBJ' x 'INVS' Ei Eo 'WITH' x1 , .. , xn 'PRE'  [ u , .. , v ] 'PROP' ( Px ; .. ; Py ) 'PARAMS' () 'GLOBALS' ( Gx ; .. ; Gy ) 'SEP' ( S1x ; .. ; S1y ) '|' S2 'POST' [ tz ] 'PROP' () 'LOCAL' () 'SEP' ( SPx ; .. ; SPy ) '|' ( SQx ; .. ; SQy )" :=
+Notation "'ATOMIC' 'TYPE' W 'OBJ' x 'INVS' E 'WITH' x1 , .. , xn 'PRE'  [ u , .. , v ] 'PROP' ( Px ; .. ; Py ) 'PARAMS' () 'GLOBALS' ( Gx ; .. ; Gy ) 'SEP' ( S1x ; .. ; S1y ) '|' S2 'POST' [ tz ] 'PROP' () 'LOCAL' () 'SEP' ( SPx ; .. ; SPy ) '|' ( SQx ; .. ; SQy )" :=
   (mk_funspec (pair (cons u%type .. (cons v%type nil) ..) tz) cc_default (atomic_spec_type0 W)
    (fun (ts: list Type) => rev_curry (tcurry (fun x1 => .. (tcurry (fun xn => tcurry (fun Q : mpred => tcurry (fun (_ : tuple_type tnil) =>
      PROPx (cons Px%type .. (cons Py%type nil) ..)
      (PARAMSx nil (GLOBALSx (cons Gx .. (cons Gy nil) ..)
-     (SEPx (cons (atomic_shift(B := unit) (fun x => S2) Ei Eo (fun x _ => fold_right_sepcon (cons SQx%logic .. (cons SQy%logic nil) ..)) (fun _ => Q)) (cons S1x%logic .. (cons S1y%logic nil) ..))))))))) ..)))
+     (SEPx (cons (atomic_shift(B := unit) (fun x => S2) (⊤ ∖ E) ∅ (fun x _ => fold_right_sepcon (cons SQx%logic .. (cons SQy%logic nil) ..)) (fun _ => Q)) (cons S1x%logic .. (cons S1y%logic nil) ..))))))))) ..)))
    (fun (ts: list Type) => rev_curry (tcurry (fun x1 => .. (tcurry (fun xn => tcurry (fun Q : mpred => tcurry (fun (_ : tuple_type tnil) =>
      PROP () LOCAL () (SEPx (Q :: cons SPx .. (cons SPy nil) ..)))))) ..)))
    (@atomic_spec_nonexpansive_pre0 _ W
@@ -879,21 +827,20 @@ Notation "'ATOMIC' 'TYPE' W 'OBJ' x 'INVS' Ei Eo 'WITH' x1 , .. , xn 'PRE'  [ u 
       (fun (ts: list Type) => rev_curry (tcurry (fun x1 => .. (tcurry (fun xn (_ : tuple_type tnil) => nil)) ..)))
       (fun (ts: list Type) => rev_curry (tcurry (fun x1 => .. (tcurry (fun xn (_ : tuple_type tnil) => (cons Gx .. (cons Gy nil) ..))) ..)))
       (fun (ts: list Type) => rev_curry (tcurry (fun x1 => .. (tcurry (fun xn (_ : tuple_type tnil) => (cons S1x%logic .. (cons S1y%logic nil) ..))) ..)))
-      (fun (ts: list Type) => rev_curry (tcurry (fun x1 => .. (tcurry (fun xn (_ : tuple_type tnil) x => S2)) ..)))
-      Ei Eo
+      (fun (ts: list Type) => rev_curry (tcurry (fun x1 => .. (tcurry (fun xn (_ : tuple_type tnil) x => S2)) ..))) E
       (fun (ts: list Type) => rev_curry (tcurry (fun x1 => .. (tcurry (fun xn (_ : tuple_type tnil) x _ => fold_right_sepcon (cons SQx%logic .. (cons SQy%logic nil) ..))) ..)))
      _ _ _ _ _ _)
   (atomic_spec_nonexpansive_post0 W
       (fun (ts: list Type) => rev_curry (tcurry (fun x1 => .. (tcurry (fun xn (_ : tuple_type tnil) => nil)) ..)))
       (fun (ts: list Type) => rev_curry (tcurry (fun x1 => .. (tcurry (fun xn (_ : tuple_type tnil) => (cons SPx%assert5%assert3 .. (cons SPy%assert5%assert3 nil) ..))) ..))) _ _))
-  (at level 200, x1 closed binder, xn closed binder, x at level 0, Ei at level 0, Eo at level 0, S2 at level 0).
+  (at level 200, x1 closed binder, xn closed binder, x at level 0, E at level 0, S2 at level 0).
 
-Notation "'ATOMIC' 'TYPE' W 'OBJ' x 'INVS' Ei Eo 'WITH' x1 , .. , xn 'PRE'  [ ] 'PROP' ( Px ; .. ; Py ) 'PARAMS' () 'GLOBALS' ( Gx ; .. ; Gy ) 'SEP' ( S1x ; .. ; S1y ) '|' S2 'POST' [ tz ] 'EX' r : T , 'PROP' () 'LOCAL' ( LQx ; .. ; LQy ) 'SEP' ( SPx ; .. ; SPy ) '|' ( SQx ; .. ; SQy )" :=
+Notation "'ATOMIC' 'TYPE' W 'OBJ' x 'INVS' E 'WITH' x1 , .. , xn 'PRE'  [ ] 'PROP' ( Px ; .. ; Py ) 'PARAMS' () 'GLOBALS' ( Gx ; .. ; Gy ) 'SEP' ( S1x ; .. ; S1y ) '|' S2 'POST' [ tz ] 'EX' r : T , 'PROP' () 'LOCAL' ( LQx ; .. ; LQy ) 'SEP' ( SPx ; .. ; SPy ) '|' ( SQx ; .. ; SQy )" :=
   (mk_funspec (pair nil tz) cc_default (atomic_spec_type W T)
    (fun (ts: list Type) => rev_curry (tcurry (fun x1 => .. (tcurry (fun xn => tcurry (fun Q : (T -> mpred) => tcurry (fun (_ : tuple_type tnil) =>
      PROPx (cons Px%type .. (cons Py%type nil) ..)
      (PARAMSx nil (GLOBALSx (cons Gx .. (cons Gy nil) ..)
-     (SEPx (cons (atomic_shift (fun x => S2) Ei Eo (fun x r => fold_right_sepcon (cons SQx%logic .. (cons SQy%logic nil) ..)) Q) (cons S1x%logic .. (cons S1y%logic nil) ..))))))))) ..)))
+     (SEPx (cons (atomic_shift (fun x => S2) (⊤ ∖ E) ∅ (fun x r => fold_right_sepcon (cons SQx%logic .. (cons SQy%logic nil) ..)) Q) (cons S1x%logic .. (cons S1y%logic nil) ..))))))))) ..)))
    (fun (ts: list Type) => rev_curry (tcurry (fun x1 => .. (tcurry (fun xn => tcurry (fun Q : (T -> mpred) => tcurry (fun (_ : tuple_type tnil) =>
     @exp (environ -> mpred) _ T (fun r =>
      PROP () (LOCALx (cons LQx .. (cons LQy nil) ..) ((SEPx (Q r :: cons SPx .. (cons SPy nil) ..))))))))) ..)))
@@ -902,21 +849,20 @@ Notation "'ATOMIC' 'TYPE' W 'OBJ' x 'INVS' Ei Eo 'WITH' x1 , .. , xn 'PRE'  [ ] 
       (fun (ts: list Type) => rev_curry (tcurry (fun x1 => .. (tcurry (fun xn (_ : tuple_type tnil) => nil)) ..)))
       (fun (ts: list Type) => rev_curry (tcurry (fun x1 => .. (tcurry (fun xn (_ : tuple_type tnil) => (cons Gx .. (cons Gy nil) ..))) ..)))
       (fun (ts: list Type) => rev_curry (tcurry (fun x1 => .. (tcurry (fun xn (_ : tuple_type tnil) => (cons S1x%logic .. (cons S1y%logic nil) ..))) ..)))
-      (fun (ts: list Type) => rev_curry (tcurry (fun x1 => .. (tcurry (fun xn (_ : tuple_type tnil) x => S2)) ..)))
-      Ei Eo
+      (fun (ts: list Type) => rev_curry (tcurry (fun x1 => .. (tcurry (fun xn (_ : tuple_type tnil) x => S2)) ..))) E
       (fun (ts: list Type) => rev_curry (tcurry (fun x1 => .. (tcurry (fun xn (_ : tuple_type tnil) x r => fold_right_sepcon (cons SQx%logic .. (cons SQy%logic nil) ..))) ..)))
      _ _ _ _ _ _)
   (atomic_spec_nonexpansive_post' W
       (fun (ts: list Type) => rev_curry (tcurry (fun x1 => .. (tcurry (fun xn (_ : tuple_type tnil) r => (cons LQx%assert3 .. (cons LQy%assert3 nil) ..))) ..)))
       (fun (ts: list Type) => rev_curry (tcurry (fun x1 => .. (tcurry (fun xn (_ : tuple_type tnil) r => (cons SPx%assert3 .. (cons SPy%assert3 nil) ..))) ..))) _ _))
-  (at level 200, x1 closed binder, xn closed binder, x at level 0, Ei at level 0, Eo at level 0, S2 at level 0, r at level 0, T at level 0).
+  (at level 200, x1 closed binder, xn closed binder, x at level 0, E at level 0, S2 at level 0, r at level 0, T at level 0).
 
-Notation "'ATOMIC' 'TYPE' W 'OBJ' x 'INVS' Ei Eo 'WITH' x1 , .. , xn 'PRE'  [ ] 'PROP' ( Px ; .. ; Py ) 'PARAMS' () 'GLOBALS' ( Gx ; .. ; Gy ) 'SEP' ( S1x ; .. ; S1y ) '|' S2 'POST' [ tz ] 'EX' r : T , 'PROP' () 'LOCAL' () 'SEP' ( SPx ; .. ; SPy ) '|' ( SQx ; .. ; SQy )" :=
+Notation "'ATOMIC' 'TYPE' W 'OBJ' x 'INVS' E 'WITH' x1 , .. , xn 'PRE'  [ ] 'PROP' ( Px ; .. ; Py ) 'PARAMS' () 'GLOBALS' ( Gx ; .. ; Gy ) 'SEP' ( S1x ; .. ; S1y ) '|' S2 'POST' [ tz ] 'EX' r : T , 'PROP' () 'LOCAL' () 'SEP' ( SPx ; .. ; SPy ) '|' ( SQx ; .. ; SQy )" :=
   (mk_funspec (pair nil tz) cc_default (atomic_spec_type W T)
    (fun (ts: list Type) => rev_curry (tcurry (fun x1 => .. (tcurry (fun xn => tcurry (fun Q : (T -> mpred) => tcurry (fun (_ : tuple_type tnil) =>
      PROPx (cons Px%type .. (cons Py%type nil) ..)
      (PARAMSx nil (GLOBALSx (cons Gx .. (cons Gy nil) ..)
-     (SEPx (cons (atomic_shift (fun x => S2) Ei Eo (fun x r => fold_right_sepcon (cons SQx%logic .. (cons SQy%logic nil) ..)) Q) (cons S1x%logic .. (cons S1y%logic nil) ..))))))))) ..)))
+     (SEPx (cons (atomic_shift (fun x => S2) (⊤ ∖ E) ∅ (fun x r => fold_right_sepcon (cons SQx%logic .. (cons SQy%logic nil) ..)) Q) (cons S1x%logic .. (cons S1y%logic nil) ..))))))))) ..)))
    (fun (ts: list Type) => rev_curry (tcurry (fun x1 => .. (tcurry (fun xn => tcurry (fun Q : (T -> mpred) => tcurry (fun (_ : tuple_type tnil) =>
     @exp (environ -> mpred) _ T (fun r =>
      PROP () (LOCAL () (SEPx (Q r :: cons SPx .. (cons SPy nil) ..)))))))) ..)))
@@ -925,21 +871,20 @@ Notation "'ATOMIC' 'TYPE' W 'OBJ' x 'INVS' Ei Eo 'WITH' x1 , .. , xn 'PRE'  [ ] 
       (fun (ts: list Type) => rev_curry (tcurry (fun x1 => .. (tcurry (fun xn (_ : tuple_type tnil) => nil)) ..)))
       (fun (ts: list Type) => rev_curry (tcurry (fun x1 => .. (tcurry (fun xn (_ : tuple_type tnil) => (cons Gx .. (cons Gy nil) ..))) ..)))
       (fun (ts: list Type) => rev_curry (tcurry (fun x1 => .. (tcurry (fun xn (_ : tuple_type tnil) => (cons S1x%logic .. (cons S1y%logic nil) ..))) ..)))
-      (fun (ts: list Type) => rev_curry (tcurry (fun x1 => .. (tcurry (fun xn (_ : tuple_type tnil) x => S2)) ..)))
-      Ei Eo
+      (fun (ts: list Type) => rev_curry (tcurry (fun x1 => .. (tcurry (fun xn (_ : tuple_type tnil) x => S2)) ..))) E
       (fun (ts: list Type) => rev_curry (tcurry (fun x1 => .. (tcurry (fun xn (_ : tuple_type tnil) x r => fold_right_sepcon (cons SQx%logic .. (cons SQy%logic nil) ..))) ..)))
      _ _ _ _ _ _)
   (atomic_spec_nonexpansive_post' W
       (fun (ts: list Type) => rev_curry (tcurry (fun x1 => .. (tcurry (fun xn (_ : tuple_type tnil) r => nil)) ..)))
       (fun (ts: list Type) => rev_curry (tcurry (fun x1 => .. (tcurry (fun xn (_ : tuple_type tnil) r => (cons SPx%assert5%assert3 .. (cons SPy%assert5%assert3 nil) ..))) ..))) _ _))
-  (at level 200, x1 closed binder, xn closed binder, x at level 0, Ei at level 0, Eo at level 0, S2 at level 0, r at level 0, T at level 0).
+  (at level 200, x1 closed binder, xn closed binder, x at level 0, E at level 0, S2 at level 0, r at level 0, T at level 0).
 
-Notation "'ATOMIC' 'TYPE' W 'OBJ' x 'INVS' Ei Eo 'WITH' x1 , .. , xn 'PRE'  [ ] 'PROP' ( Px ; .. ; Py ) 'PARAMS () 'GLOBALS' ( Gx ; .. ; Gy ) 'SEP' ( S1x ; .. ; S1y ) '|' S2 'POST' [ tz ] 'PROP' () 'LOCAL' ( LQx ; .. ; LQy ) 'SEP' ( SPx ; .. ; SPy ) '|' ( SQx ; .. ; SQy )" :=
+Notation "'ATOMIC' 'TYPE' W 'OBJ' x 'INVS' E 'WITH' x1 , .. , xn 'PRE'  [ ] 'PROP' ( Px ; .. ; Py ) 'PARAMS () 'GLOBALS' ( Gx ; .. ; Gy ) 'SEP' ( S1x ; .. ; S1y ) '|' S2 'POST' [ tz ] 'PROP' () 'LOCAL' ( LQx ; .. ; LQy ) 'SEP' ( SPx ; .. ; SPy ) '|' ( SQx ; .. ; SQy )" :=
   (mk_funspec (pair nil tz) cc_default (atomic_spec_type0 W)
    (fun (ts: list Type) => rev_curry (tcurry (fun x1 => .. (tcurry (fun xn => tcurry (fun Q : mpred => tcurry (fun (_ : tuple_type tnil) =>
      PROPx (cons Px%type .. (cons Py%type nil) ..)
      (PARAMSx nil (GLOBALSx (cons Gx .. (cons Gy nil) ..)
-     (SEPx (cons (atomic_shift(B := unit) (fun x => S2) Ei Eo (fun x _ => fold_right_sepcon (cons SQx%logic .. (cons SQy%logic nil) ..)) (fun _ => Q)) (cons S1x%logic .. (cons S1y%logic nil) ..))))))))) ..)))
+     (SEPx (cons (atomic_shift(B := unit) (fun x => S2) (⊤ ∖ E) ∅ (fun x _ => fold_right_sepcon (cons SQx%logic .. (cons SQy%logic nil) ..)) (fun _ => Q)) (cons S1x%logic .. (cons S1y%logic nil) ..))))))))) ..)))
    (fun (ts: list Type) => rev_curry (tcurry (fun x1 => .. (tcurry (fun xn => tcurry (fun Q : mpred => tcurry (fun (_ : tuple_type tnil) =>
      PROP () LOCAL () (SEPx (Q :: cons SPx .. (cons SPy nil) ..)))))) ..)))
    (@atomic_spec_nonexpansive_pre0 _ W
@@ -947,21 +892,20 @@ Notation "'ATOMIC' 'TYPE' W 'OBJ' x 'INVS' Ei Eo 'WITH' x1 , .. , xn 'PRE'  [ ] 
       (fun (ts: list Type) => rev_curry (tcurry (fun x1 => .. (tcurry (fun xn (_ : tuple_type tnil) => nil)) ..)))
       (fun (ts: list Type) => rev_curry (tcurry (fun x1 => .. (tcurry (fun xn (_ : tuple_type tnil) => (cons Gx .. (cons Gy nil) ..))) ..)))
       (fun (ts: list Type) => rev_curry (tcurry (fun x1 => .. (tcurry (fun xn (_ : tuple_type tnil) => (cons S1x%logic .. (cons S1y%logic nil) ..))) ..)))
-      (fun (ts: list Type) => rev_curry (tcurry (fun x1 => .. (tcurry (fun xn (_ : tuple_type tnil) x => S2)) ..)))
-      Ei Eo
+      (fun (ts: list Type) => rev_curry (tcurry (fun x1 => .. (tcurry (fun xn (_ : tuple_type tnil) x => S2)) ..))) E
       (fun (ts: list Type) => rev_curry (tcurry (fun x1 => .. (tcurry (fun xn (_ : tuple_type tnil) x _ => fold_right_sepcon (cons SQx%logic .. (cons SQy%logic nil) ..))) ..)))
      _ _ _ _ _ _)
   (atomic_spec_nonexpansive_post0 W
       (fun (ts: list Type) => rev_curry (tcurry (fun x1 => .. (tcurry (fun xn (_ : tuple_type tnil) => (cons LQx%logic .. (cons LQy%logic nil) ..))) ..)))
       (fun (ts: list Type) => rev_curry (tcurry (fun x1 => .. (tcurry (fun xn (_ : tuple_type tnil) => (cons SPx%assert5%assert3 .. (cons SPy%assert5%assert3 nil) ..))) ..))) _ _))
-  (at level 200, x1 closed binder, xn closed binder, x at level 0, Ei at level 0, Eo at level 0, S2 at level 0).
+  (at level 200, x1 closed binder, xn closed binder, x at level 0, E at level 0, S2 at level 0).
 
-Notation "'ATOMIC' 'TYPE' W 'OBJ' x 'INVS' Ei Eo 'WITH' x1 , .. , xn 'PRE'  [ ] 'PROP' ( Px ; .. ; Py ) 'PARAMS' () 'GLOBALS' ( Gx ; .. ; Gy ) 'SEP' ( S1x ; .. ; S1y ) '|' S2 'POST' [ tz ] 'PROP' () 'LOCAL' () 'SEP' ( SPx ; .. ; SPy ) '|' ( SQx ; .. ; SQy )" :=
+Notation "'ATOMIC' 'TYPE' W 'OBJ' x 'INVS' E 'WITH' x1 , .. , xn 'PRE'  [ ] 'PROP' ( Px ; .. ; Py ) 'PARAMS' () 'GLOBALS' ( Gx ; .. ; Gy ) 'SEP' ( S1x ; .. ; S1y ) '|' S2 'POST' [ tz ] 'PROP' () 'LOCAL' () 'SEP' ( SPx ; .. ; SPy ) '|' ( SQx ; .. ; SQy )" :=
   (mk_funspec (pair nil tz) cc_default (atomic_spec_type0 W)
    (fun (ts: list Type) => rev_curry (tcurry (fun x1 => .. (tcurry (fun xn => tcurry (fun Q : mpred => tcurry (fun (_ : tuple_type tnil) =>
      PROPx (cons Px%type .. (cons Py%type nil) ..)
      (PARAMSx nil (GLOBALSx (cons Gx .. (cons Gy nil) ..)
-     (SEPx (cons (atomic_shift(B := unit) (fun x => S2) Ei Eo (fun x _ => fold_right_sepcon (cons SQx%logic .. (cons SQy%logic nil) ..)) (fun _ => Q)) (cons S1x%logic .. (cons S1y%logic nil) ..))))))))) ..)))
+     (SEPx (cons (atomic_shift(B := unit) (fun x => S2) (⊤ ∖ E) ∅ (fun x _ => fold_right_sepcon (cons SQx%logic .. (cons SQy%logic nil) ..)) (fun _ => Q)) (cons S1x%logic .. (cons S1y%logic nil) ..))))))))) ..)))
    (fun (ts: list Type) => rev_curry (tcurry (fun x1 => .. (tcurry (fun xn => tcurry (fun Q : mpred => tcurry (fun (_ : tuple_type tnil) =>
      PROP () LOCAL () (SEPx (Q :: cons SPx .. (cons SPy nil) ..)))))) ..)))
    (@atomic_spec_nonexpansive_pre0 _ W
@@ -969,21 +913,20 @@ Notation "'ATOMIC' 'TYPE' W 'OBJ' x 'INVS' Ei Eo 'WITH' x1 , .. , xn 'PRE'  [ ] 
       (fun (ts: list Type) => rev_curry (tcurry (fun x1 => .. (tcurry (fun xn (_ : tuple_type tnil) => nil)) ..)))
       (fun (ts: list Type) => rev_curry (tcurry (fun x1 => .. (tcurry (fun xn (_ : tuple_type tnil) => (cons Gx .. (cons Gy nil) ..))) ..)))
       (fun (ts: list Type) => rev_curry (tcurry (fun x1 => .. (tcurry (fun xn (_ : tuple_type tnil) => (cons S1x%logic .. (cons S1y%logic nil) ..))) ..)))
-      (fun (ts: list Type) => rev_curry (tcurry (fun x1 => .. (tcurry (fun xn (_ : tuple_type tnil) x => S2)) ..)))
-      Ei Eo
+      (fun (ts: list Type) => rev_curry (tcurry (fun x1 => .. (tcurry (fun xn (_ : tuple_type tnil) x => S2)) ..))) E
       (fun (ts: list Type) => rev_curry (tcurry (fun x1 => .. (tcurry (fun xn (_ : tuple_type tnil) x _ => fold_right_sepcon (cons SQx%logic .. (cons SQy%logic nil) ..))) ..)))
      _ _ _ _ _ _)
   (atomic_spec_nonexpansive_post0 W
       (fun (ts: list Type) => rev_curry (tcurry (fun x1 => .. (tcurry (fun xn (_ : tuple_type tnil) => nil)) ..)))
       (fun (ts: list Type) => rev_curry (tcurry (fun x1 => .. (tcurry (fun xn (_ : tuple_type tnil) => (cons SPx%assert5%assert3 .. (cons SPy%assert5%assert3 nil) ..))) ..))) _ _))
-  (at level 200, x1 closed binder, xn closed binder, x at level 0, Ei at level 0, Eo at level 0, S2 at level 0).
+  (at level 200, x1 closed binder, xn closed binder, x at level 0, E at level 0, S2 at level 0).
 
-Notation "'ATOMIC' 'TYPE' W 'INVS' Ei Eo 'WITH' x1 , .. , xn 'PRE'  [ u , .. , v ] 'PROP' () 'PARAMS' ( Lx ; .. ; Ly ) 'GLOBALS' ( Gx ; .. ; Gy ) 'SEP' ( S1x ; .. ; S1y ) '|' S2 'POST' [ tz ] 'PROP' () 'LOCAL' () 'SEP' ( SPx ; .. ; SPy ) '|' ( SQx ; .. ; SQy )" :=
+Notation "'ATOMIC' 'TYPE' W 'INVS' E 'WITH' x1 , .. , xn 'PRE'  [ u , .. , v ] 'PROP' () 'PARAMS' ( Lx ; .. ; Ly ) 'GLOBALS' ( Gx ; .. ; Gy ) 'SEP' ( S1x ; .. ; S1y ) '|' S2 'POST' [ tz ] 'PROP' () 'LOCAL' () 'SEP' ( SPx ; .. ; SPy ) '|' ( SQx ; .. ; SQy )" :=
   (mk_funspec (pair (cons u%type .. (cons v%type nil) ..) tz) cc_default (atomic_spec_type0 W)
    (fun (ts: list Type) => rev_curry (tcurry (fun x1 => .. (tcurry (fun xn => tcurry (fun Q : mpred => tcurry (fun (_ : tuple_type tnil) =>
      PROPx nil
      (PARAMSx (cons Lx%type .. (cons Ly%type nil) ..) (GLOBALSx (cons Gx .. (cons Gy nil) ..)
-     (SEPx (cons (atomic_shift(B := unit) (fun _ : unit => S2) Ei Eo (fun _ _ => fold_right_sepcon (cons SQx%logic .. (cons SQy%logic nil) ..)) (fun _ => Q)) (cons S1x%logic .. (cons S1y%logic nil) ..))))))))) ..)))
+     (SEPx (cons (atomic_shift(B := unit) (fun _ : unit => S2) (⊤ ∖ E) ∅ (fun _ _ => fold_right_sepcon (cons SQx%logic .. (cons SQy%logic nil) ..)) (fun _ => Q)) (cons S1x%logic .. (cons S1y%logic nil) ..))))))))) ..)))
    (fun (ts: list Type) => rev_curry (tcurry (fun x1 => .. (tcurry (fun xn => tcurry (fun Q : mpred => tcurry (fun (_ : tuple_type tnil) =>
      PROP () LOCAL () (SEPx (Q :: cons SPx .. (cons SPy nil) ..)))))) ..)))
    (@atomic_spec_nonexpansive_pre0 _ W
@@ -991,21 +934,20 @@ Notation "'ATOMIC' 'TYPE' W 'INVS' Ei Eo 'WITH' x1 , .. , xn 'PRE'  [ u , .. , v
       (fun (ts: list Type) => rev_curry (tcurry (fun x1 => .. (tcurry (fun xn (_ : tuple_type tnil) => (cons Lx%type .. (cons Ly%type nil) ..))) ..)))
       (fun (ts: list Type) => rev_curry (tcurry (fun x1 => .. (tcurry (fun xn (_ : tuple_type tnil) => (cons Gx .. (cons Gy nil) ..))) ..)))
       (fun (ts: list Type) => rev_curry (tcurry (fun x1 => .. (tcurry (fun xn (_ : tuple_type tnil) => (cons S1x%logic .. (cons S1y%logic nil) ..))) ..)))
-      (fun (ts: list Type) => rev_curry (tcurry (fun x1 => .. (tcurry (fun xn (_ : tuple_type tnil) (_:unit) => S2)) ..)))
-      Ei Eo
+      (fun (ts: list Type) => rev_curry (tcurry (fun x1 => .. (tcurry (fun xn (_ : tuple_type tnil) (_:unit) => S2)) ..))) E
       (fun (ts: list Type) => rev_curry (tcurry (fun x1 => .. (tcurry (fun xn (_ : tuple_type tnil) _ _ => fold_right_sepcon (cons SQx%logic .. (cons SQy%logic nil) ..))) ..)))
      _ _ _ _ _ _)
   (atomic_spec_nonexpansive_post0 W
       (fun (ts: list Type) => rev_curry (tcurry (fun x1 => .. (tcurry (fun xn (_ : tuple_type tnil) => nil)) ..)))
       (fun (ts: list Type) => rev_curry (tcurry (fun x1 => .. (tcurry (fun xn (_ : tuple_type tnil) => (cons SPx%assert5%assert3 .. (cons SPy%assert5%assert3 nil) ..))) ..))) _ _))
-  (at level 200, x1 closed binder, xn closed binder, Ei at level 0, Eo at level 0, S2 at level 0).
+  (at level 200, x1 closed binder, xn closed binder, E at level 0, S2 at level 0).
 
-Notation "'ATOMIC' 'TYPE' W 'OBJ' x 'INVS' Ei Eo 'WITH' x1 , .. , xn 'PRE'  [ u , .. , v ] 'PROP' () 'PARAMS' ( Lx ; .. ; Ly ) 'GLOBALS' ( Gx ; .. ; Gy ) 'SEP' ( S1x ; .. ; S1y ) '|' S2 'POST' [ tz ] 'PROP' () 'LOCAL' () 'SEP' ( SPx ; .. ; SPy ) '|' ( SQx ; .. ; SQy )" :=
+Notation "'ATOMIC' 'TYPE' W 'OBJ' x 'INVS' E 'WITH' x1 , .. , xn 'PRE'  [ u , .. , v ] 'PROP' () 'PARAMS' ( Lx ; .. ; Ly ) 'GLOBALS' ( Gx ; .. ; Gy ) 'SEP' ( S1x ; .. ; S1y ) '|' S2 'POST' [ tz ] 'PROP' () 'LOCAL' () 'SEP' ( SPx ; .. ; SPy ) '|' ( SQx ; .. ; SQy )" :=
   (mk_funspec (pair (cons u%type .. (cons v%type nil) ..) tz) cc_default (atomic_spec_type0 W)
    (fun (ts: list Type) => rev_curry (tcurry (fun x1 => .. (tcurry (fun xn => tcurry (fun Q : mpred => tcurry (fun (_ : tuple_type tnil) =>
      PROPx nil
      (PARAMSx (cons Lx%type .. (cons Ly%type nil) ..) (GLOBALSx (cons Gx .. (cons Gy nil) ..)
-     (SEPx (cons (atomic_shift(B := unit) (fun x => S2) Ei Eo (fun x _ => fold_right_sepcon (cons SQx%logic .. (cons SQy%logic nil) ..)) (fun _ => Q)) (cons S1x%logic .. (cons S1y%logic nil) ..))))))))) ..)))
+     (SEPx (cons (atomic_shift(B := unit) (fun x => S2) (⊤ ∖ E) ∅ (fun x _ => fold_right_sepcon (cons SQx%logic .. (cons SQy%logic nil) ..)) (fun _ => Q)) (cons S1x%logic .. (cons S1y%logic nil) ..))))))))) ..)))
    (fun (ts: list Type) => rev_curry (tcurry (fun x1 => .. (tcurry (fun xn => tcurry (fun Q : mpred => tcurry (fun (_ : tuple_type tnil) =>
      PROP () LOCAL () (SEPx (Q :: cons SPx .. (cons SPy nil) ..)))))) ..)))
    (@atomic_spec_nonexpansive_pre0 _ W
@@ -1013,14 +955,13 @@ Notation "'ATOMIC' 'TYPE' W 'OBJ' x 'INVS' Ei Eo 'WITH' x1 , .. , xn 'PRE'  [ u 
       (fun (ts: list Type) => rev_curry (tcurry (fun x1 => .. (tcurry (fun xn (_ : tuple_type tnil) => (cons Lx%type .. (cons Ly%type nil) ..))) ..)))
       (fun (ts: list Type) => rev_curry (tcurry (fun x1 => .. (tcurry (fun xn (_ : tuple_type tnil) => (cons Gx .. (cons Gy nil) ..))) ..)))
       (fun (ts: list Type) => rev_curry (tcurry (fun x1 => .. (tcurry (fun xn (_ : tuple_type tnil) => (cons S1x%logic .. (cons S1y%logic nil) ..))) ..)))
-      (fun (ts: list Type) => rev_curry (tcurry (fun x1 => .. (tcurry (fun xn (_ : tuple_type tnil) x => S2)) ..)))
-      Ei Eo
+      (fun (ts: list Type) => rev_curry (tcurry (fun x1 => .. (tcurry (fun xn (_ : tuple_type tnil) x => S2)) ..))) E
       (fun (ts: list Type) => rev_curry (tcurry (fun x1 => .. (tcurry (fun xn (_ : tuple_type tnil) x _ => fold_right_sepcon (cons SQx%logic .. (cons SQy%logic nil) ..))) ..)))
      _ _ _ _ _ _)
   (atomic_spec_nonexpansive_post0 W
       (fun (ts: list Type) => rev_curry (tcurry (fun x1 => .. (tcurry (fun xn (_ : tuple_type tnil) => nil)) ..)))
       (fun (ts: list Type) => rev_curry (tcurry (fun x1 => .. (tcurry (fun xn (_ : tuple_type tnil) => (cons SPx%assert5%assert3 .. (cons SPy%assert5%assert3 nil) ..))) ..))) _ _))
-  (at level 200, x1 closed binder, xn closed binder, x at level 0, Ei at level 0, Eo at level 0, S2 at level 0).
+  (at level 200, x1 closed binder, xn closed binder, x at level 0, E at level 0, S2 at level 0).
 
 Ltac atomic_nonexpansive_tac := try (let x := fresh "x" in intros ?? x;
   try match type of x with list Type => (let ts := fresh "ts" in rename x into ts; intros x) end;
